Improved presentation, documentation.

src/Corecursive_Prop.thy
@@ -1,4 +1,5 @@
-chapter\<open>Equivalence of Operational and Denotational Semantics\<close>
+(*chapter\<open>Equivalence of Operational and Denotational Semantics\<close>*)
+text\<open>\chapter[Semantics Equivalence]{Equivalence of Operational and Denotational Semantics}\<close>
 
 theory Corecursive_Prop
   imports
@@ -12,74 +13,81 @@ section \<open>Stepwise denotational interpretation of TESL atoms\<close>
 
 text \<open> Denotational interpretation of TESL bounded by index\<close>
 fun TESL_interpretation_atomic_stepwise
-    :: \<open>('\<tau>::linordered_field) TESL_atomic \<Rightarrow> nat \<Rightarrow> '\<tau> run set\<close> ("\<lbrakk> _ \<rbrakk>\<^sub>T\<^sub>E\<^sub>S\<^sub>L\<^bsup>\<ge> _\<^esup>") where
-    \<open>\<lbrakk> K\<^sub>1 sporadic \<tau> on K\<^sub>2 \<rbrakk>\<^sub>T\<^sub>E\<^sub>S\<^sub>L\<^bsup>\<ge> i\<^esup> =
-        { \<rho>. \<exists>n\<ge>i. hamlet ((Rep_run \<rho>) n K\<^sub>1) = True \<and> time ((Rep_run \<rho>) n K\<^sub>2) = \<tau> }\<close>
-  | \<open>\<lbrakk> time-relation \<lfloor>K\<^sub>1, K\<^sub>2\<rfloor> \<in> R \<rbrakk>\<^sub>T\<^sub>E\<^sub>S\<^sub>L\<^bsup>\<ge> i\<^esup> =
-        { \<rho>. \<forall>n\<ge>i. R (time ((Rep_run \<rho>) n K\<^sub>1), time ((Rep_run \<rho>) n K\<^sub>2)) }\<close>
-  | \<open>\<lbrakk> master implies slave \<rbrakk>\<^sub>T\<^sub>E\<^sub>S\<^sub>L\<^bsup>\<ge> i\<^esup> =
-        { \<rho>. \<forall>n\<ge>i. hamlet ((Rep_run \<rho>) n master) \<longrightarrow> hamlet ((Rep_run \<rho>) n slave) }\<close>
-  | \<open>\<lbrakk> master implies not slave \<rbrakk>\<^sub>T\<^sub>E\<^sub>S\<^sub>L\<^bsup>\<ge> i\<^esup> =
-        { \<rho>. \<forall>n\<ge>i. hamlet ((Rep_run \<rho>) n master) \<longrightarrow> \<not> hamlet ((Rep_run \<rho>) n slave) }\<close>
-  | \<open>\<lbrakk> master time-delayed by \<delta>\<tau> on measuring implies slave \<rbrakk>\<^sub>T\<^sub>E\<^sub>S\<^sub>L\<^bsup>\<ge> i\<^esup> =
-        { \<rho>. \<forall>n\<ge>i. hamlet ((Rep_run \<rho>) n master) \<longrightarrow>
-                 (let measured_time = time ((Rep_run \<rho>) n measuring) in
-                  \<forall>m \<ge> n. first_time \<rho> measuring m (measured_time + \<delta>\<tau>)
-                           \<longrightarrow> hamlet ((Rep_run \<rho>) m slave)
-                 )
-        }\<close>
-  | \<open>\<lbrakk> K\<^sub>1 weakly precedes K\<^sub>2 \<rbrakk>\<^sub>T\<^sub>E\<^sub>S\<^sub>L\<^bsup>\<ge> i\<^esup> =
-        { \<rho>. \<forall>n\<ge>i. (run_tick_count \<rho> K\<^sub>2 n) \<le> (run_tick_count \<rho> K\<^sub>1 n) }\<close>
-  | \<open>\<lbrakk> K\<^sub>1 strictly precedes K\<^sub>2 \<rbrakk>\<^sub>T\<^sub>E\<^sub>S\<^sub>L\<^bsup>\<ge> i\<^esup> =
-        { \<rho>. \<forall>n\<ge>i. (run_tick_count \<rho> K\<^sub>2 n) \<le> (run_tick_count_strictly \<rho> K\<^sub>1 n) }\<close>
-  | \<open>\<lbrakk> K\<^sub>1 kills K\<^sub>2 \<rbrakk>\<^sub>T\<^sub>E\<^sub>S\<^sub>L\<^bsup>\<ge> i\<^esup> =
-        { \<rho>. \<forall>n\<ge>i. hamlet ((Rep_run \<rho>) n K\<^sub>1) \<longrightarrow> (\<forall>m\<ge>n. \<not> hamlet ((Rep_run \<rho>) m K\<^sub>2)) }\<close>
+    :: \<open>('\<tau>::linordered_field) TESL_atomic \<Rightarrow> nat \<Rightarrow> '\<tau> run set\<close> ("\<lbrakk> _ \<rbrakk>\<^sub>T\<^sub>E\<^sub>S\<^sub>L\<^bsup>\<ge> _\<^esup>")
+where
+  \<open>\<lbrakk> K\<^sub>1 sporadic \<tau> on K\<^sub>2 \<rbrakk>\<^sub>T\<^sub>E\<^sub>S\<^sub>L\<^bsup>\<ge> i\<^esup> =
+      {\<rho>. \<exists>n\<ge>i. hamlet ((Rep_run \<rho>) n K\<^sub>1) = True \<and> time ((Rep_run \<rho>) n K\<^sub>2) = \<tau>}\<close>
+| \<open>\<lbrakk> time-relation \<lfloor>K\<^sub>1, K\<^sub>2\<rfloor> \<in> R \<rbrakk>\<^sub>T\<^sub>E\<^sub>S\<^sub>L\<^bsup>\<ge> i\<^esup> =
+      {\<rho>. \<forall>n\<ge>i. R (time ((Rep_run \<rho>) n K\<^sub>1), time ((Rep_run \<rho>) n K\<^sub>2))}\<close>
+| \<open>\<lbrakk> master implies slave \<rbrakk>\<^sub>T\<^sub>E\<^sub>S\<^sub>L\<^bsup>\<ge> i\<^esup> =
+      {\<rho>. \<forall>n\<ge>i. hamlet ((Rep_run \<rho>) n master) \<longrightarrow> hamlet ((Rep_run \<rho>) n slave)}\<close>
+| \<open>\<lbrakk> master implies not slave \<rbrakk>\<^sub>T\<^sub>E\<^sub>S\<^sub>L\<^bsup>\<ge> i\<^esup> =
+      {\<rho>. \<forall>n\<ge>i. hamlet ((Rep_run \<rho>) n master) \<longrightarrow> \<not> hamlet ((Rep_run \<rho>) n slave)}\<close>
+| \<open>\<lbrakk> master time-delayed by \<delta>\<tau> on measuring implies slave \<rbrakk>\<^sub>T\<^sub>E\<^sub>S\<^sub>L\<^bsup>\<ge> i\<^esup> =
+      {\<rho>. \<forall>n\<ge>i. hamlet ((Rep_run \<rho>) n master) \<longrightarrow>
+               (let measured_time = time ((Rep_run \<rho>) n measuring) in
+                \<forall>m \<ge> n. first_time \<rho> measuring m (measured_time + \<delta>\<tau>)
+                         \<longrightarrow> hamlet ((Rep_run \<rho>) m slave)
+               )
+      }\<close>
+| \<open>\<lbrakk> K\<^sub>1 weakly precedes K\<^sub>2 \<rbrakk>\<^sub>T\<^sub>E\<^sub>S\<^sub>L\<^bsup>\<ge> i\<^esup> =
+      {\<rho>. \<forall>n\<ge>i. (run_tick_count \<rho> K\<^sub>2 n) \<le> (run_tick_count \<rho> K\<^sub>1 n)}\<close>
+| \<open>\<lbrakk> K\<^sub>1 strictly precedes K\<^sub>2 \<rbrakk>\<^sub>T\<^sub>E\<^sub>S\<^sub>L\<^bsup>\<ge> i\<^esup> =
+      {\<rho>. \<forall>n\<ge>i. (run_tick_count \<rho> K\<^sub>2 n) \<le> (run_tick_count_strictly \<rho> K\<^sub>1 n)}\<close>
+| \<open>\<lbrakk> K\<^sub>1 kills K\<^sub>2 \<rbrakk>\<^sub>T\<^sub>E\<^sub>S\<^sub>L\<^bsup>\<ge> i\<^esup> =
+      {\<rho>. \<forall>n\<ge>i. hamlet ((Rep_run \<rho>) n K\<^sub>1) \<longrightarrow> (\<forall>m\<ge>n. \<not> hamlet ((Rep_run \<rho>) m K\<^sub>2))}\<close>
 
 
 theorem predicate_Inter_unfold:
-  \<open>{ \<rho>. \<forall>n. P \<rho> n} = \<Inter> {Y. \<exists>n. Y = { \<rho>. P \<rho> n }}\<close>
-  by (simp add: Collect_all_eq full_SetCompr_eq)
+  \<open>{\<rho>. \<forall>n. P \<rho> n} = \<Inter> {Y. \<exists>n. Y = {\<rho>. P \<rho> n}}\<close>
+by (simp add: Collect_all_eq full_SetCompr_eq)
 
 theorem predicate_Union_unfold:
-  \<open>{ \<rho>. \<exists>n. P \<rho> n} = \<Union> {Y. \<exists>n. Y = { \<rho>. P \<rho> n }}\<close>
-  by auto
+  \<open>{\<rho>. \<exists>n. P \<rho> n} = \<Union> {Y. \<exists>n. Y = {\<rho>. P \<rho> n}}\<close>
+by auto
 
 lemma TESL_interp_unfold_stepwise_sporadicon:
-  shows \<open>\<lbrakk> K\<^sub>1 sporadic \<tau> on K\<^sub>2 \<rbrakk>\<^sub>T\<^sub>E\<^sub>S\<^sub>L = \<Union> {Y. \<exists>n::nat. Y = \<lbrakk> K\<^sub>1 sporadic \<tau> on K\<^sub>2 \<rbrakk>\<^sub>T\<^sub>E\<^sub>S\<^sub>L\<^bsup>\<ge> n\<^esup>}\<close>
-  by auto
+  \<open>\<lbrakk> K\<^sub>1 sporadic \<tau> on K\<^sub>2 \<rbrakk>\<^sub>T\<^sub>E\<^sub>S\<^sub>L = \<Union> {Y. \<exists>n::nat. Y = \<lbrakk> K\<^sub>1 sporadic \<tau> on K\<^sub>2 \<rbrakk>\<^sub>T\<^sub>E\<^sub>S\<^sub>L\<^bsup>\<ge> n\<^esup>}\<close>
+by auto
 
 lemma TESL_interp_unfold_stepwise_tagrelgen:
-  shows \<open>\<lbrakk> time-relation \<lfloor>K\<^sub>1, K\<^sub>2\<rfloor> \<in> R \<rbrakk>\<^sub>T\<^sub>E\<^sub>S\<^sub>L = \<Inter> {Y. \<exists>n::nat. Y = \<lbrakk> time-relation \<lfloor>K\<^sub>1, K\<^sub>2\<rfloor> \<in> R \<rbrakk>\<^sub>T\<^sub>E\<^sub>S\<^sub>L\<^bsup>\<ge> n\<^esup>}\<close>
-  by auto
+  \<open>\<lbrakk> time-relation \<lfloor>K\<^sub>1, K\<^sub>2\<rfloor> \<in> R \<rbrakk>\<^sub>T\<^sub>E\<^sub>S\<^sub>L
+    = \<Inter> {Y. \<exists>n::nat. Y = \<lbrakk> time-relation \<lfloor>K\<^sub>1, K\<^sub>2\<rfloor> \<in> R \<rbrakk>\<^sub>T\<^sub>E\<^sub>S\<^sub>L\<^bsup>\<ge> n\<^esup>}\<close>
+by auto
 
 lemma TESL_interp_unfold_stepwise_implies:
-  shows \<open>\<lbrakk> master implies slave \<rbrakk>\<^sub>T\<^sub>E\<^sub>S\<^sub>L = \<Inter> {Y. \<exists>n::nat. Y = \<lbrakk> master implies slave \<rbrakk>\<^sub>T\<^sub>E\<^sub>S\<^sub>L\<^bsup>\<ge> n\<^esup>}\<close>
-  by auto
+  \<open>\<lbrakk> master implies slave \<rbrakk>\<^sub>T\<^sub>E\<^sub>S\<^sub>L
+    = \<Inter> {Y. \<exists>n::nat. Y = \<lbrakk> master implies slave \<rbrakk>\<^sub>T\<^sub>E\<^sub>S\<^sub>L\<^bsup>\<ge> n\<^esup>}\<close>
+by auto
 
 lemma TESL_interp_unfold_stepwise_implies_not:
-  shows \<open>\<lbrakk> master implies not slave \<rbrakk>\<^sub>T\<^sub>E\<^sub>S\<^sub>L = \<Inter> {Y. \<exists>n::nat. Y = \<lbrakk> master implies not slave \<rbrakk>\<^sub>T\<^sub>E\<^sub>S\<^sub>L\<^bsup>\<ge> n\<^esup>}\<close>
-  by auto
+  \<open>\<lbrakk> master implies not slave \<rbrakk>\<^sub>T\<^sub>E\<^sub>S\<^sub>L
+    = \<Inter> {Y. \<exists>n::nat. Y = \<lbrakk> master implies not slave \<rbrakk>\<^sub>T\<^sub>E\<^sub>S\<^sub>L\<^bsup>\<ge> n\<^esup>}\<close>
+by auto
 
 lemma TESL_interp_unfold_stepwise_timedelayed:
-  shows \<open>\<lbrakk> master time-delayed by \<delta>\<tau> on measuring implies slave \<rbrakk>\<^sub>T\<^sub>E\<^sub>S\<^sub>L
+  \<open>\<lbrakk> master time-delayed by \<delta>\<tau> on measuring implies slave \<rbrakk>\<^sub>T\<^sub>E\<^sub>S\<^sub>L
     = \<Inter> {Y. \<exists>n::nat. Y = \<lbrakk> master time-delayed by \<delta>\<tau> on measuring implies slave \<rbrakk>\<^sub>T\<^sub>E\<^sub>S\<^sub>L\<^bsup>\<ge> n\<^esup>}\<close>
-  by auto
+by auto
 
 lemma TESL_interp_unfold_stepwise_weakly_precedes:
-  shows \<open>\<lbrakk> K\<^sub>1 weakly precedes K\<^sub>2 \<rbrakk>\<^sub>T\<^sub>E\<^sub>S\<^sub>L = \<Inter> {Y. \<exists>n::nat. Y = \<lbrakk> K\<^sub>1 weakly precedes K\<^sub>2 \<rbrakk>\<^sub>T\<^sub>E\<^sub>S\<^sub>L\<^bsup>\<ge> n\<^esup>}\<close>
-  by auto
+  \<open>\<lbrakk> K\<^sub>1 weakly precedes K\<^sub>2 \<rbrakk>\<^sub>T\<^sub>E\<^sub>S\<^sub>L
+    = \<Inter> {Y. \<exists>n::nat. Y = \<lbrakk> K\<^sub>1 weakly precedes K\<^sub>2 \<rbrakk>\<^sub>T\<^sub>E\<^sub>S\<^sub>L\<^bsup>\<ge> n\<^esup>}\<close>
+by auto
 
 lemma TESL_interp_unfold_stepwise_strictly_precedes:
-  shows \<open>\<lbrakk> K\<^sub>1 strictly precedes K\<^sub>2 \<rbrakk>\<^sub>T\<^sub>E\<^sub>S\<^sub>L = \<Inter> {Y. \<exists>n::nat. Y = \<lbrakk> K\<^sub>1 strictly precedes K\<^sub>2 \<rbrakk>\<^sub>T\<^sub>E\<^sub>S\<^sub>L\<^bsup>\<ge> n\<^esup>}\<close>
-  by auto
+  \<open>\<lbrakk> K\<^sub>1 strictly precedes K\<^sub>2 \<rbrakk>\<^sub>T\<^sub>E\<^sub>S\<^sub>L
+    = \<Inter> {Y. \<exists>n::nat. Y = \<lbrakk> K\<^sub>1 strictly precedes K\<^sub>2 \<rbrakk>\<^sub>T\<^sub>E\<^sub>S\<^sub>L\<^bsup>\<ge> n\<^esup>}\<close>
+by auto
 
 lemma TESL_interp_unfold_stepwise_kills:
-  shows \<open>\<lbrakk> master kills slave \<rbrakk>\<^sub>T\<^sub>E\<^sub>S\<^sub>L = \<Inter> {Y. \<exists>n::nat. Y = \<lbrakk> master kills slave \<rbrakk>\<^sub>T\<^sub>E\<^sub>S\<^sub>L\<^bsup>\<ge> n\<^esup>}\<close>
-  by auto
+  \<open>\<lbrakk> master kills slave \<rbrakk>\<^sub>T\<^sub>E\<^sub>S\<^sub>L = \<Inter> {Y. \<exists>n::nat. Y = \<lbrakk> master kills slave \<rbrakk>\<^sub>T\<^sub>E\<^sub>S\<^sub>L\<^bsup>\<ge> n\<^esup>}\<close>
+by auto
 
 theorem TESL_interp_unfold_stepwise_positive_atoms:
   assumes \<open>positive_atom \<phi>\<close>
-  shows \<open>\<lbrakk> \<phi>::'\<tau>::linordered_field TESL_atomic \<rbrakk>\<^sub>T\<^sub>E\<^sub>S\<^sub>L = \<Union> {Y. \<exists>n::nat. Y = \<lbrakk> \<phi> \<rbrakk>\<^sub>T\<^sub>E\<^sub>S\<^sub>L\<^bsup>\<ge> n\<^esup>}\<close>
+  shows \<open>\<lbrakk> \<phi>::'\<tau>::linordered_field TESL_atomic \<rbrakk>\<^sub>T\<^sub>E\<^sub>S\<^sub>L
+          = \<Union> {Y. \<exists>n::nat. Y = \<lbrakk> \<phi> \<rbrakk>\<^sub>T\<^sub>E\<^sub>S\<^sub>L\<^bsup>\<ge> n\<^esup>}\<close>
 proof -
   from positive_atom.elims(2)[OF assms]
     obtain u v w where \<open>\<phi> = (u sporadic v on w)\<close> by blast
@@ -92,35 +100,36 @@ theorem TESL_interp_unfold_stepwise_negative_atoms:
 proof (cases \<phi>)
   case SporadicOn thus ?thesis using assms by simp
 next
-  case (TagRelation x41 x42 x43)
-  thus ?thesis using TESL_interp_unfold_stepwise_tagrelgen by simp
+  case TagRelation
+    thus ?thesis using TESL_interp_unfold_stepwise_tagrelgen by simp
 next
-  case (Implies x51 x52)
-  thus ?thesis using TESL_interp_unfold_stepwise_implies by simp
+  case Implies
+    thus ?thesis using TESL_interp_unfold_stepwise_implies by simp
 next
-  case (ImpliesNot x51 x52)
-  thus ?thesis using TESL_interp_unfold_stepwise_implies_not by simp
+  case ImpliesNot
+    thus ?thesis using TESL_interp_unfold_stepwise_implies_not by simp
 next
-  case (TimeDelayedBy x61 x62 x63 x64)
-  thus ?thesis using TESL_interp_unfold_stepwise_timedelayed by simp
+  case TimeDelayedBy
+    thus ?thesis using TESL_interp_unfold_stepwise_timedelayed by simp
 next
-  case (WeaklyPrecedes x61 x62)
-  then show ?thesis
-    using TESL_interp_unfold_stepwise_weakly_precedes by simp
+  case WeaklyPrecedes
+    thus ?thesis
+      using TESL_interp_unfold_stepwise_weakly_precedes by simp
 next
-  case (StrictlyPrecedes x61 x62)
-  then show ?thesis
-    using TESL_interp_unfold_stepwise_strictly_precedes by simp
+  case StrictlyPrecedes
+    thus ?thesis
+      using TESL_interp_unfold_stepwise_strictly_precedes by simp
 next
-  case (Kills x63 x64)
-  then show ?thesis
-    using TESL_interp_unfold_stepwise_kills by simp
+  case Kills
+    thus ?thesis
+      using TESL_interp_unfold_stepwise_kills by simp
 qed
 
 lemma forall_nat_expansion:
   \<open>(\<forall>n \<ge> (n\<^sub>0::nat). P n) = (P n\<^sub>0 \<and> (\<forall>n \<ge> Suc n\<^sub>0. P n))\<close>
 proof -
-  have \<open>(\<forall>n \<ge> (n\<^sub>0::nat). P n) = (\<forall>n. (n = n\<^sub>0 \<or> n > n\<^sub>0) \<longrightarrow> P n)\<close> using le_less by blast
+  have \<open>(\<forall>n \<ge> (n\<^sub>0::nat). P n) = (\<forall>n. (n = n\<^sub>0 \<or> n > n\<^sub>0) \<longrightarrow> P n)\<close>
+    using le_less by blast
   also have \<open>... = (P n\<^sub>0 \<and> (\<forall>n > n\<^sub>0. P n))\<close> by blast
   finally show ?thesis using Suc_le_eq by simp
 qed
@@ -128,46 +137,40 @@ qed
 lemma exists_nat_expansion:
   \<open>(\<exists>n \<ge> (n\<^sub>0::nat). P n) = (P n\<^sub>0 \<or> (\<exists>n \<ge> Suc n\<^sub>0. P n))\<close>
 proof -
-  have \<open>(\<exists>n \<ge> (n\<^sub>0::nat). P n) = (\<exists>n. (n = n\<^sub>0 \<or> n > n\<^sub>0) \<and> P n)\<close> using le_less by blast
+  have \<open>(\<exists>n \<ge> (n\<^sub>0::nat). P n) = (\<exists>n. (n = n\<^sub>0 \<or> n > n\<^sub>0) \<and> P n)\<close>
+    using le_less by blast
   also have \<open>... = (\<exists>n. (P n\<^sub>0) \<or> (n > n\<^sub>0 \<and> P n))\<close> by blast
   finally show ?thesis using Suc_le_eq by simp
 qed
 
 section \<open>Coinduction Unfolding Properties\<close>
 
-lemma TESL_interp_stepwise_sporadicon_cst_coind_unfold:
-  shows \<open>\<lbrakk> K\<^sub>1 sporadic \<tau> on K\<^sub>2 \<rbrakk>\<^sub>T\<^sub>E\<^sub>S\<^sub>L\<^bsup>\<ge> n\<^esup> =
-    \<lbrakk> K\<^sub>1 \<Up> n \<rbrakk>\<^sub>p\<^sub>r\<^sub>i\<^sub>m \<inter> \<lbrakk> K\<^sub>2 \<Down> n @ \<tau> \<rbrakk>\<^sub>p\<^sub>r\<^sub>i\<^sub>m
-    \<union> \<lbrakk> K\<^sub>1 sporadic \<tau> on K\<^sub>2 \<rbrakk>\<^sub>T\<^sub>E\<^sub>S\<^sub>L\<^bsup>\<ge> Suc n\<^esup>\<close>
-  proof -
-    have \<open>{ \<rho>. \<exists>m\<ge>n. hamlet ((Rep_run \<rho>) m K\<^sub>1) = True \<and> time ((Rep_run \<rho>) m K\<^sub>2) = \<tau> }
-        = { \<rho>. hamlet ((Rep_run \<rho>) n K\<^sub>1) = True \<and> time ((Rep_run \<rho>) n K\<^sub>2) = \<tau>
-               \<or> (\<exists>m\<ge>Suc n. hamlet ((Rep_run \<rho>) m K\<^sub>1) = True \<and> time ((Rep_run \<rho>) m K\<^sub>2) = \<tau>) }\<close>
-      using Suc_leD not_less_eq_eq by fastforce
-    moreover have \<open>{ \<rho>. hamlet ((Rep_run \<rho>) n K\<^sub>1) = True \<and> time ((Rep_run \<rho>) n K\<^sub>2) = \<tau>
-                        \<or> (\<exists>m\<ge>Suc n. hamlet ((Rep_run \<rho>) m K\<^sub>1) = True \<and> time ((Rep_run \<rho>) m K\<^sub>2) = \<tau>) }
-                 = \<lbrakk> K\<^sub>1 \<Up> n \<rbrakk>\<^sub>p\<^sub>r\<^sub>i\<^sub>m \<inter> \<lbrakk> K\<^sub>2 \<Down> n @ \<tau> \<rbrakk>\<^sub>p\<^sub>r\<^sub>i\<^sub>m \<union> \<lbrakk> K\<^sub>1 sporadic \<tau> on K\<^sub>2 \<rbrakk>\<^sub>T\<^sub>E\<^sub>S\<^sub>L\<^bsup>\<ge> Suc n\<^esup>\<close>
-      by (simp add: Collect_conj_eq Collect_disj_eq)
-    ultimately show ?thesis by auto
-  qed
-
 lemma TESL_interp_stepwise_sporadicon_coind_unfold:
-  shows \<open>\<lbrakk> K\<^sub>1 sporadic \<tau> on K\<^sub>2 \<rbrakk>\<^sub>T\<^sub>E\<^sub>S\<^sub>L\<^bsup>\<ge> n\<^esup> =
+  \<open>\<lbrakk> K\<^sub>1 sporadic \<tau> on K\<^sub>2 \<rbrakk>\<^sub>T\<^sub>E\<^sub>S\<^sub>L\<^bsup>\<ge> n\<^esup> =
     \<lbrakk> K\<^sub>1 \<Up> n \<rbrakk>\<^sub>p\<^sub>r\<^sub>i\<^sub>m \<inter> \<lbrakk> K\<^sub>2 \<Down> n @ \<tau> \<rbrakk>\<^sub>p\<^sub>r\<^sub>i\<^sub>m
     \<union> \<lbrakk> K\<^sub>1 sporadic \<tau> on K\<^sub>2 \<rbrakk>\<^sub>T\<^sub>E\<^sub>S\<^sub>L\<^bsup>\<ge> Suc n\<^esup>\<close>
-  using TESL_interp_stepwise_sporadicon_cst_coind_unfold by blast
+proof -
+  have \<open>{\<rho>. \<exists>m\<ge>n. hamlet ((Rep_run \<rho>) m K\<^sub>1) = True \<and> time ((Rep_run \<rho>) m K\<^sub>2) = \<tau>}
+    = {\<rho>. hamlet ((Rep_run \<rho>) n K\<^sub>1) = True \<and> time ((Rep_run \<rho>) n K\<^sub>2) = \<tau>
+      \<or> (\<exists>m\<ge>Suc n. hamlet ((Rep_run \<rho>) m K\<^sub>1) = True \<and> time ((Rep_run \<rho>) m K\<^sub>2) = \<tau>)}\<close>
+    using Suc_leD not_less_eq_eq by fastforce
+  moreover have
+    \<open>{\<rho>. hamlet ((Rep_run \<rho>) n K\<^sub>1) \<and> time ((Rep_run \<rho>) n K\<^sub>2) = \<tau>
+       \<or> (\<exists>m\<ge>Suc n. hamlet ((Rep_run \<rho>) m K\<^sub>1) \<and> time ((Rep_run \<rho>) m K\<^sub>2) = \<tau>)}
+    = \<lbrakk> K\<^sub>1 \<Up> n \<rbrakk>\<^sub>p\<^sub>r\<^sub>i\<^sub>m \<inter> \<lbrakk> K\<^sub>2 \<Down> n @ \<tau> \<rbrakk>\<^sub>p\<^sub>r\<^sub>i\<^sub>m \<union> \<lbrakk> K\<^sub>1 sporadic \<tau> on K\<^sub>2 \<rbrakk>\<^sub>T\<^sub>E\<^sub>S\<^sub>L\<^bsup>\<ge> Suc n\<^esup>\<close>
+    by (simp add: Collect_conj_eq Collect_disj_eq)
+  ultimately show ?thesis by auto
+qed
 
 lemma nat_set_suc:\<open>{x. \<forall>m \<ge> n. P x m} = {x. P x n} \<inter> {x. \<forall>m \<ge> Suc n. P x m}\<close>
 proof
-  { fix x
-    assume h:\<open>x \<in> {x. \<forall>m \<ge> n. P x m}\<close>
+    { fix x assume h:\<open>x \<in> {x. \<forall>m \<ge> n. P x m}\<close>
     hence \<open>P x n\<close> by simp
     moreover from h have \<open>x \<in> {x. \<forall>m \<ge> Suc n. P x m}\<close> by simp
     ultimately have \<open>x \<in> {x. P x n} \<inter> {x. \<forall>m \<ge> Suc n. P x m}\<close> by simp
   } thus \<open>{x. \<forall>m \<ge> n. P x m} \<subseteq> {x. P x n} \<inter> {x. \<forall>m \<ge> Suc n. P x m}\<close> ..
 next
-  { fix x
-    assume h:\<open>x \<in> {x. P x n} \<inter> {x. \<forall>m \<ge> Suc n. P x m}\<close>
+  { fix x  assume h:\<open>x \<in> {x. P x n} \<inter> {x. \<forall>m \<ge> Suc n. P x m}\<close>
     hence \<open>P x n\<close> by simp
     moreover from h have \<open>\<forall>m \<ge> Suc n. P x m\<close> by simp
     ultimately have \<open>\<forall>m \<ge> n. P x m\<close> using forall_nat_expansion by blast
@@ -176,92 +179,102 @@ next
 qed
 
 lemma TESL_interp_stepwise_tagrel_coind_unfold:
-  shows \<open>\<lbrakk> time-relation \<lfloor>K\<^sub>1, K\<^sub>2\<rfloor> \<in> R \<rbrakk>\<^sub>T\<^sub>E\<^sub>S\<^sub>L\<^bsup>\<ge> n\<^esup> =
-    \<lbrakk> \<lfloor>\<tau>\<^sub>v\<^sub>a\<^sub>r(K\<^sub>1, n), \<tau>\<^sub>v\<^sub>a\<^sub>r(K\<^sub>2, n)\<rfloor> \<in> R \<rbrakk>\<^sub>p\<^sub>r\<^sub>i\<^sub>m
-    \<inter> \<lbrakk> time-relation \<lfloor>K\<^sub>1, K\<^sub>2\<rfloor> \<in> R \<rbrakk>\<^sub>T\<^sub>E\<^sub>S\<^sub>L\<^bsup>\<ge> Suc n\<^esup>\<close>
+  \<open>\<lbrakk> time-relation \<lfloor>K\<^sub>1, K\<^sub>2\<rfloor> \<in> R \<rbrakk>\<^sub>T\<^sub>E\<^sub>S\<^sub>L\<^bsup>\<ge> n\<^esup> =
+     \<lbrakk> \<lfloor>\<tau>\<^sub>v\<^sub>a\<^sub>r(K\<^sub>1, n), \<tau>\<^sub>v\<^sub>a\<^sub>r(K\<^sub>2, n)\<rfloor> \<in> R \<rbrakk>\<^sub>p\<^sub>r\<^sub>i\<^sub>m
+     \<inter> \<lbrakk> time-relation \<lfloor>K\<^sub>1, K\<^sub>2\<rfloor> \<in> R \<rbrakk>\<^sub>T\<^sub>E\<^sub>S\<^sub>L\<^bsup>\<ge> Suc n\<^esup>\<close>
 proof -
-  have \<open>{ \<rho>. \<forall>m\<ge>n. R (time ((Rep_run \<rho>) m K\<^sub>1), time ((Rep_run \<rho>) m K\<^sub>2)) }
-       = { \<rho>. R (time ((Rep_run \<rho>) n K\<^sub>1), time ((Rep_run \<rho>) n K\<^sub>2)) }
-       \<inter> { \<rho>. \<forall>m\<ge>Suc n. R (time ((Rep_run \<rho>) m K\<^sub>1), time ((Rep_run \<rho>) m K\<^sub>2)) }\<close>
-    using nat_set_suc[of \<open>n\<close> \<open>\<lambda>x y. R (time ((Rep_run x) y K\<^sub>1), time ((Rep_run x) y K\<^sub>2))\<close>] by simp
-  then show ?thesis by auto
+  have \<open>{\<rho>. \<forall>m\<ge>n. R (time ((Rep_run \<rho>) m K\<^sub>1), time ((Rep_run \<rho>) m K\<^sub>2))}
+       = {\<rho>. R (time ((Rep_run \<rho>) n K\<^sub>1), time ((Rep_run \<rho>) n K\<^sub>2))}
+       \<inter> {\<rho>. \<forall>m\<ge>Suc n. R (time ((Rep_run \<rho>) m K\<^sub>1), time ((Rep_run \<rho>) m K\<^sub>2))}\<close>
+    using nat_set_suc[of \<open>n\<close> \<open>\<lambda>x y. R (time ((Rep_run x) y K\<^sub>1),
+                                       time ((Rep_run x) y K\<^sub>2))\<close>] by simp
+  thus ?thesis by auto
 qed
 
 lemma TESL_interp_stepwise_implies_coind_unfold:
-  shows \<open>\<lbrakk> master implies slave \<rbrakk>\<^sub>T\<^sub>E\<^sub>S\<^sub>L\<^bsup>\<ge> n\<^esup> =
-    (\<lbrakk> master \<not>\<Up> n \<rbrakk>\<^sub>p\<^sub>r\<^sub>i\<^sub>m \<union> \<lbrakk> master \<Up> n \<rbrakk>\<^sub>p\<^sub>r\<^sub>i\<^sub>m \<inter> \<lbrakk> slave \<Up> n \<rbrakk>\<^sub>p\<^sub>r\<^sub>i\<^sub>m)
-    \<inter> \<lbrakk> master implies slave \<rbrakk>\<^sub>T\<^sub>E\<^sub>S\<^sub>L\<^bsup>\<ge> Suc n\<^esup>\<close>
+  \<open>\<lbrakk> master implies slave \<rbrakk>\<^sub>T\<^sub>E\<^sub>S\<^sub>L\<^bsup>\<ge> n\<^esup> =
+     (\<lbrakk> master \<not>\<Up> n \<rbrakk>\<^sub>p\<^sub>r\<^sub>i\<^sub>m \<union> \<lbrakk> master \<Up> n \<rbrakk>\<^sub>p\<^sub>r\<^sub>i\<^sub>m \<inter> \<lbrakk> slave \<Up> n \<rbrakk>\<^sub>p\<^sub>r\<^sub>i\<^sub>m)
+     \<inter> \<lbrakk> master implies slave \<rbrakk>\<^sub>T\<^sub>E\<^sub>S\<^sub>L\<^bsup>\<ge> Suc n\<^esup>\<close>
 proof -
-  have \<open>{ \<rho>. \<forall>m\<ge>n. hamlet ((Rep_run \<rho>) m master) \<longrightarrow> hamlet ((Rep_run \<rho>) m slave) }
-        = { \<rho>. hamlet ((Rep_run \<rho>) n master) \<longrightarrow> hamlet ((Rep_run \<rho>) n slave) }
-        \<inter> { \<rho>. \<forall>m\<ge>Suc n. hamlet ((Rep_run \<rho>) m master) \<longrightarrow> hamlet ((Rep_run \<rho>) m slave) }\<close>
-    using nat_set_suc[of \<open>n\<close> \<open>\<lambda>x y. hamlet ((Rep_run x) y master) \<longrightarrow> hamlet ((Rep_run x) y slave)\<close>] by simp
-  then show ?thesis by auto
+  have \<open>{\<rho>. \<forall>m\<ge>n. hamlet ((Rep_run \<rho>) m master) \<longrightarrow> hamlet ((Rep_run \<rho>) m slave)}
+        = {\<rho>. hamlet ((Rep_run \<rho>) n master) \<longrightarrow> hamlet ((Rep_run \<rho>) n slave)}
+        \<inter> {\<rho>. \<forall>m\<ge>Suc n. hamlet ((Rep_run \<rho>) m master)
+                     \<longrightarrow> hamlet ((Rep_run \<rho>) m slave)}\<close>
+    using nat_set_suc[of \<open>n\<close> \<open>\<lambda>x y. hamlet ((Rep_run x) y master)
+                                \<longrightarrow> hamlet ((Rep_run x) y slave)\<close>] by simp
+  thus ?thesis by auto
 qed
 
 lemma TESL_interp_stepwise_implies_not_coind_unfold:
-  shows \<open>\<lbrakk> master implies not slave \<rbrakk>\<^sub>T\<^sub>E\<^sub>S\<^sub>L\<^bsup>\<ge> n\<^esup> =
-    (\<lbrakk> master \<not>\<Up> n \<rbrakk>\<^sub>p\<^sub>r\<^sub>i\<^sub>m \<union> \<lbrakk> master \<Up> n \<rbrakk>\<^sub>p\<^sub>r\<^sub>i\<^sub>m \<inter> \<lbrakk> slave \<not>\<Up> n \<rbrakk>\<^sub>p\<^sub>r\<^sub>i\<^sub>m)
-    \<inter> \<lbrakk> master implies not slave \<rbrakk>\<^sub>T\<^sub>E\<^sub>S\<^sub>L\<^bsup>\<ge> Suc n\<^esup>\<close>
+  \<open>\<lbrakk> master implies not slave \<rbrakk>\<^sub>T\<^sub>E\<^sub>S\<^sub>L\<^bsup>\<ge> n\<^esup> =
+     (\<lbrakk> master \<not>\<Up> n \<rbrakk>\<^sub>p\<^sub>r\<^sub>i\<^sub>m \<union> \<lbrakk> master \<Up> n \<rbrakk>\<^sub>p\<^sub>r\<^sub>i\<^sub>m \<inter> \<lbrakk> slave \<not>\<Up> n \<rbrakk>\<^sub>p\<^sub>r\<^sub>i\<^sub>m)
+     \<inter> \<lbrakk> master implies not slave \<rbrakk>\<^sub>T\<^sub>E\<^sub>S\<^sub>L\<^bsup>\<ge> Suc n\<^esup>\<close>
 proof -
-  have \<open>{ \<rho>. \<forall>m\<ge>n. hamlet ((Rep_run \<rho>) m master) \<longrightarrow> \<not> hamlet ((Rep_run \<rho>) m slave) }
-        = { \<rho>. hamlet ((Rep_run \<rho>) n master) \<longrightarrow> \<not> hamlet ((Rep_run \<rho>) n slave) }
-        \<inter> { \<rho>. \<forall>m\<ge>Suc n. hamlet ((Rep_run \<rho>) m master) \<longrightarrow> \<not> hamlet ((Rep_run \<rho>) m slave) }\<close>
-    using nat_set_suc[of \<open>n\<close> \<open>\<lambda>x y. hamlet ((Rep_run x) y master) \<longrightarrow> \<not> hamlet ((Rep_run x) y slave)\<close>] by simp
-  then show ?thesis by auto
+  have \<open>{\<rho>. \<forall>m\<ge>n. hamlet ((Rep_run \<rho>) m master) \<longrightarrow> \<not> hamlet ((Rep_run \<rho>) m slave)}
+       = {\<rho>. hamlet ((Rep_run \<rho>) n master) \<longrightarrow> \<not> hamlet ((Rep_run \<rho>) n slave)}
+          \<inter> {\<rho>. \<forall>m\<ge>Suc n. hamlet ((Rep_run \<rho>) m master)
+                     \<longrightarrow> \<not> hamlet ((Rep_run \<rho>) m slave)}\<close>
+    using nat_set_suc[of \<open>n\<close> \<open>\<lambda>x y. hamlet ((Rep_run x) y master)
+                               \<longrightarrow> \<not>hamlet ((Rep_run x) y slave)\<close>] by simp
+  thus ?thesis by auto
 qed
 
 lemma TESL_interp_stepwise_timedelayed_coind_unfold:
-  shows \<open>\<lbrakk> master time-delayed by \<delta>\<tau> on measuring implies slave \<rbrakk>\<^sub>T\<^sub>E\<^sub>S\<^sub>L\<^bsup>\<ge> n\<^esup> =
-    (\<lbrakk> master \<not>\<Up> n \<rbrakk>\<^sub>p\<^sub>r\<^sub>i\<^sub>m \<union> (\<lbrakk> master \<Up> n \<rbrakk>\<^sub>p\<^sub>r\<^sub>i\<^sub>m \<inter> \<lbrakk> measuring @ n \<oplus> \<delta>\<tau> \<Rightarrow> slave \<rbrakk>\<^sub>p\<^sub>r\<^sub>i\<^sub>m))
-    \<inter> \<lbrakk> master time-delayed by \<delta>\<tau> on measuring implies slave \<rbrakk>\<^sub>T\<^sub>E\<^sub>S\<^sub>L\<^bsup>\<ge> Suc n\<^esup>\<close>
+  \<open>\<lbrakk> master time-delayed by \<delta>\<tau> on measuring implies slave \<rbrakk>\<^sub>T\<^sub>E\<^sub>S\<^sub>L\<^bsup>\<ge> n\<^esup> =
+     (\<lbrakk> master \<not>\<Up> n \<rbrakk>\<^sub>p\<^sub>r\<^sub>i\<^sub>m \<union> (\<lbrakk> master \<Up> n \<rbrakk>\<^sub>p\<^sub>r\<^sub>i\<^sub>m \<inter> \<lbrakk> measuring @ n \<oplus> \<delta>\<tau> \<Rightarrow> slave \<rbrakk>\<^sub>p\<^sub>r\<^sub>i\<^sub>m))
+     \<inter> \<lbrakk> master time-delayed by \<delta>\<tau> on measuring implies slave \<rbrakk>\<^sub>T\<^sub>E\<^sub>S\<^sub>L\<^bsup>\<ge> Suc n\<^esup>\<close>
 proof -
   let ?prop = \<open>\<lambda>\<rho> m. hamlet ((Rep_run \<rho>) m master) \<longrightarrow>
                  (let measured_time = time ((Rep_run \<rho>) m measuring) in
                   \<forall>p \<ge> m. first_time \<rho> measuring p (measured_time + \<delta>\<tau>)
                            \<longrightarrow> hamlet ((Rep_run \<rho>) p slave))\<close>
-  have \<open>{ \<rho>. \<forall>m \<ge> n. ?prop \<rho> m} = { \<rho>. ?prop \<rho> n} \<inter> {\<rho>. \<forall>m \<ge> Suc n. ?prop \<rho> m}\<close>
+  have \<open>{\<rho>. \<forall>m \<ge> n. ?prop \<rho> m} = {\<rho>. ?prop \<rho> n} \<inter> {\<rho>. \<forall>m \<ge> Suc n. ?prop \<rho> m}\<close>
     using nat_set_suc[of \<open>n\<close> ?prop] by blast
-  also have \<open>... = { \<rho>. ?prop \<rho> n } \<inter> \<lbrakk> master time-delayed by \<delta>\<tau> on measuring implies slave \<rbrakk>\<^sub>T\<^sub>E\<^sub>S\<^sub>L\<^bsup>\<ge> Suc n\<^esup>\<close> by simp
+  also have \<open>... = {\<rho>. ?prop \<rho> n}
+              \<inter> \<lbrakk> master time-delayed by \<delta>\<tau> on measuring implies slave \<rbrakk>\<^sub>T\<^sub>E\<^sub>S\<^sub>L\<^bsup>\<ge> Suc n\<^esup>\<close>
+    by simp
   finally show ?thesis by auto
 qed
 
 lemma TESL_interp_stepwise_weakly_precedes_coind_unfold:
-  shows \<open>\<lbrakk> K\<^sub>1 weakly precedes K\<^sub>2 \<rbrakk>\<^sub>T\<^sub>E\<^sub>S\<^sub>L\<^bsup>\<ge> n\<^esup> =
-    \<lbrakk> (\<lceil>#\<^sup>\<le> K\<^sub>2 n, #\<^sup>\<le> K\<^sub>1 n\<rceil> \<in> (\<lambda>(x,y). x\<le>y)) \<rbrakk>\<^sub>p\<^sub>r\<^sub>i\<^sub>m
-    \<inter> \<lbrakk> K\<^sub>1 weakly precedes K\<^sub>2 \<rbrakk>\<^sub>T\<^sub>E\<^sub>S\<^sub>L\<^bsup>\<ge> Suc n\<^esup>\<close>
+   \<open>\<lbrakk> K\<^sub>1 weakly precedes K\<^sub>2 \<rbrakk>\<^sub>T\<^sub>E\<^sub>S\<^sub>L\<^bsup>\<ge> n\<^esup> =
+      \<lbrakk> (\<lceil>#\<^sup>\<le> K\<^sub>2 n, #\<^sup>\<le> K\<^sub>1 n\<rceil> \<in> (\<lambda>(x,y). x\<le>y)) \<rbrakk>\<^sub>p\<^sub>r\<^sub>i\<^sub>m
+      \<inter> \<lbrakk> K\<^sub>1 weakly precedes K\<^sub>2 \<rbrakk>\<^sub>T\<^sub>E\<^sub>S\<^sub>L\<^bsup>\<ge> Suc n\<^esup>\<close>
 proof -
-  have \<open>{ \<rho>. \<forall>p\<ge>n. (run_tick_count \<rho> K\<^sub>2 p) \<le> (run_tick_count \<rho> K\<^sub>1 p) }
-         = { \<rho>. (run_tick_count \<rho> K\<^sub>2 n) \<le> (run_tick_count \<rho> K\<^sub>1 n) }
-         \<inter> { \<rho>. \<forall>p\<ge>Suc n. (run_tick_count \<rho> K\<^sub>2 p) \<le> (run_tick_count \<rho> K\<^sub>1 p) }\<close>
-    using nat_set_suc[of \<open>n\<close> \<open>\<lambda>\<rho> n. (run_tick_count \<rho> K\<^sub>2 n) \<le> (run_tick_count \<rho> K\<^sub>1 n)\<close>]
+  have \<open>{\<rho>. \<forall>p\<ge>n. (run_tick_count \<rho> K\<^sub>2 p) \<le> (run_tick_count \<rho> K\<^sub>1 p)}
+         = {\<rho>. (run_tick_count \<rho> K\<^sub>2 n) \<le> (run_tick_count \<rho> K\<^sub>1 n)}
+         \<inter> {\<rho>. \<forall>p\<ge>Suc n. (run_tick_count \<rho> K\<^sub>2 p) \<le> (run_tick_count \<rho> K\<^sub>1 p)}\<close>
+    using nat_set_suc[of \<open>n\<close> \<open>\<lambda>\<rho> n. (run_tick_count \<rho> K\<^sub>2 n)
+                                  \<le> (run_tick_count \<rho> K\<^sub>1 n)\<close>]
     by simp
-  then show ?thesis by auto
+  thus ?thesis by auto
 qed
 
 lemma TESL_interp_stepwise_strictly_precedes_coind_unfold:
-  shows \<open>\<lbrakk> K\<^sub>1 strictly precedes K\<^sub>2 \<rbrakk>\<^sub>T\<^sub>E\<^sub>S\<^sub>L\<^bsup>\<ge> n\<^esup> =
-    \<lbrakk> (\<lceil>#\<^sup>\<le> K\<^sub>2 n, #\<^sup>< K\<^sub>1 n\<rceil> \<in> (\<lambda>(x,y). x\<le>y)) \<rbrakk>\<^sub>p\<^sub>r\<^sub>i\<^sub>m
-    \<inter> \<lbrakk> K\<^sub>1 strictly precedes K\<^sub>2 \<rbrakk>\<^sub>T\<^sub>E\<^sub>S\<^sub>L\<^bsup>\<ge> Suc n\<^esup>\<close>
+   \<open>\<lbrakk> K\<^sub>1 strictly precedes K\<^sub>2 \<rbrakk>\<^sub>T\<^sub>E\<^sub>S\<^sub>L\<^bsup>\<ge> n\<^esup> =
+      \<lbrakk> (\<lceil>#\<^sup>\<le> K\<^sub>2 n, #\<^sup>< K\<^sub>1 n\<rceil> \<in> (\<lambda>(x,y). x\<le>y)) \<rbrakk>\<^sub>p\<^sub>r\<^sub>i\<^sub>m
+      \<inter> \<lbrakk> K\<^sub>1 strictly precedes K\<^sub>2 \<rbrakk>\<^sub>T\<^sub>E\<^sub>S\<^sub>L\<^bsup>\<ge> Suc n\<^esup>\<close>
 proof -
-  have \<open>{ \<rho>. \<forall>p\<ge>n. (run_tick_count \<rho> K\<^sub>2 p) \<le> (run_tick_count_strictly \<rho> K\<^sub>1 p) }
-         = { \<rho>. (run_tick_count \<rho> K\<^sub>2 n) \<le> (run_tick_count_strictly \<rho> K\<^sub>1 n) }
-         \<inter> { \<rho>. \<forall>p\<ge>Suc n. (run_tick_count \<rho> K\<^sub>2 p) \<le> (run_tick_count_strictly \<rho> K\<^sub>1 p) }\<close>
-    using nat_set_suc[of \<open>n\<close> \<open>\<lambda>\<rho> n. (run_tick_count \<rho> K\<^sub>2 n) \<le> (run_tick_count_strictly \<rho> K\<^sub>1 n)\<close>]
+  have \<open>{\<rho>. \<forall>p\<ge>n. (run_tick_count \<rho> K\<^sub>2 p) \<le> (run_tick_count_strictly \<rho> K\<^sub>1 p)}
+         = {\<rho>. (run_tick_count \<rho> K\<^sub>2 n) \<le> (run_tick_count_strictly \<rho> K\<^sub>1 n)}
+         \<inter> {\<rho>. \<forall>p\<ge>Suc n. (run_tick_count \<rho> K\<^sub>2 p) \<le> (run_tick_count_strictly \<rho> K\<^sub>1 p)}\<close>
+    using nat_set_suc[of \<open>n\<close> \<open>\<lambda>\<rho> n. (run_tick_count \<rho> K\<^sub>2 n)
+                                  \<le> (run_tick_count_strictly \<rho> K\<^sub>1 n)\<close>]
     by simp
-  then show ?thesis by auto
+  thus ?thesis by auto
 qed
 
 lemma TESL_interp_stepwise_kills_coind_unfold:
-  shows \<open>\<lbrakk> K\<^sub>1 kills K\<^sub>2 \<rbrakk>\<^sub>T\<^sub>E\<^sub>S\<^sub>L\<^bsup>\<ge> n\<^esup> =
-    (\<lbrakk> K\<^sub>1 \<not>\<Up> n \<rbrakk>\<^sub>p\<^sub>r\<^sub>i\<^sub>m \<union> \<lbrakk> K\<^sub>1 \<Up> n \<rbrakk>\<^sub>p\<^sub>r\<^sub>i\<^sub>m \<inter> \<lbrakk> K\<^sub>2 \<not>\<Up> \<ge> n \<rbrakk>\<^sub>p\<^sub>r\<^sub>i\<^sub>m)
-    \<inter> \<lbrakk> K\<^sub>1 kills K\<^sub>2 \<rbrakk>\<^sub>T\<^sub>E\<^sub>S\<^sub>L\<^bsup>\<ge> Suc n\<^esup>\<close>
+   \<open>\<lbrakk> K\<^sub>1 kills K\<^sub>2 \<rbrakk>\<^sub>T\<^sub>E\<^sub>S\<^sub>L\<^bsup>\<ge> n\<^esup> =
+      (\<lbrakk> K\<^sub>1 \<not>\<Up> n \<rbrakk>\<^sub>p\<^sub>r\<^sub>i\<^sub>m \<union> \<lbrakk> K\<^sub>1 \<Up> n \<rbrakk>\<^sub>p\<^sub>r\<^sub>i\<^sub>m \<inter> \<lbrakk> K\<^sub>2 \<not>\<Up> \<ge> n \<rbrakk>\<^sub>p\<^sub>r\<^sub>i\<^sub>m)
+      \<inter> \<lbrakk> K\<^sub>1 kills K\<^sub>2 \<rbrakk>\<^sub>T\<^sub>E\<^sub>S\<^sub>L\<^bsup>\<ge> Suc n\<^esup>\<close>
 proof -
-  let ?kills = \<open>\<lambda>n \<rho>. \<forall>p\<ge>n. hamlet ((Rep_run \<rho>) p K\<^sub>1) \<longrightarrow> (\<forall>m\<ge>p. \<not> hamlet ((Rep_run \<rho>) m K\<^sub>2))\<close>
+  let ?kills = \<open>\<lambda>n \<rho>. \<forall>p\<ge>n. hamlet ((Rep_run \<rho>) p K\<^sub>1)
+                             \<longrightarrow> (\<forall>m\<ge>p. \<not> hamlet ((Rep_run \<rho>) m K\<^sub>2))\<close>
   let ?ticks = \<open>\<lambda>n \<rho> c. hamlet ((Rep_run \<rho>) n c)\<close>
   let ?dead = \<open>\<lambda>n \<rho> c. \<forall>m \<ge> n. \<not>hamlet ((Rep_run \<rho>) m c)\<close>
   have \<open>\<lbrakk> K\<^sub>1 kills K\<^sub>2 \<rbrakk>\<^sub>T\<^sub>E\<^sub>S\<^sub>L\<^bsup>\<ge> n\<^esup> = {\<rho>. ?kills n \<rho>}\<close> by simp
-  also have \<open>... = ({\<rho>. \<not> ?ticks n \<rho> K\<^sub>1}  \<inter> { \<rho>. ?kills (Suc n) \<rho>})
+  also have \<open>... = ({\<rho>. \<not> ?ticks n \<rho> K\<^sub>1}  \<inter> {\<rho>. ?kills (Suc n) \<rho>})
                  \<union> ({\<rho>. ?ticks n \<rho> K\<^sub>1} \<inter> {\<rho>. ?dead n \<rho> K\<^sub>2})\<close>
   proof
     { fix \<rho>::\<open>'\<tau>::linordered_field run\<close>
@@ -277,7 +290,7 @@ proof -
             \<union> {\<rho>. ?ticks n \<rho> K\<^sub>1} \<inter> {\<rho>. ?dead n \<rho> K\<^sub>2}\<close> by blast
   next
     { fix \<rho>::\<open>'\<tau>::linordered_field run\<close>
-      assume \<open>\<rho> \<in> ({\<rho>. \<not> ?ticks n \<rho> K\<^sub>1}  \<inter> { \<rho>. ?kills (Suc n) \<rho>})
+      assume \<open>\<rho> \<in> ({\<rho>. \<not> ?ticks n \<rho> K\<^sub>1}  \<inter> {\<rho>. ?kills (Suc n) \<rho>})
                  \<union> ({\<rho>. ?ticks n \<rho> K\<^sub>1} \<inter> {\<rho>. ?dead n \<rho> K\<^sub>2})\<close>
       hence \<open>\<not> ?ticks n \<rho> K\<^sub>1 \<and> ?kills (Suc n) \<rho>
              \<or> ?ticks n \<rho> K\<^sub>1 \<and> ?dead n \<rho> K\<^sub>2\<close> by blast
@@ -285,7 +298,7 @@ proof -
         using dual_order.antisym not_less_eq_eq by blast
       ultimately have \<open>?kills n \<rho> \<or> ?ticks n \<rho> K\<^sub>1 \<and> ?dead n \<rho> K\<^sub>2\<close> by blast
       hence \<open>?kills n \<rho>\<close> using le_trans by blast
-    } thus \<open>({\<rho>. \<not> ?ticks n \<rho> K\<^sub>1}  \<inter> { \<rho>. ?kills (Suc n) \<rho>})
+    } thus \<open>({\<rho>. \<not> ?ticks n \<rho> K\<^sub>1}  \<inter> {\<rho>. ?kills (Suc n) \<rho>})
                  \<union> ({\<rho>. ?ticks n \<rho> K\<^sub>1} \<inter> {\<rho>. ?dead n \<rho> K\<^sub>2})
           \<subseteq> {\<rho>. ?kills n \<rho>}\<close> by blast
   qed
@@ -293,13 +306,17 @@ proof -
                  \<union> {\<rho>. ?ticks n \<rho> K\<^sub>1} \<inter> {\<rho>. ?dead n \<rho> K\<^sub>2} \<inter> {\<rho>. ?kills (Suc n) \<rho>}\<close>
     using Collect_cong Collect_disj_eq by auto
   also have \<open>... = \<lbrakk> K\<^sub>1 \<not>\<Up> n \<rbrakk>\<^sub>p\<^sub>r\<^sub>i\<^sub>m \<inter> \<lbrakk> K\<^sub>1 kills K\<^sub>2 \<rbrakk>\<^sub>T\<^sub>E\<^sub>S\<^sub>L\<^bsup>\<ge> Suc n\<^esup>
-                 \<union> \<lbrakk> K\<^sub>1 \<Up> n \<rbrakk>\<^sub>p\<^sub>r\<^sub>i\<^sub>m \<inter> \<lbrakk> K\<^sub>2 \<not>\<Up> \<ge> n \<rbrakk>\<^sub>p\<^sub>r\<^sub>i\<^sub>m \<inter> \<lbrakk> K\<^sub>1 kills K\<^sub>2 \<rbrakk>\<^sub>T\<^sub>E\<^sub>S\<^sub>L\<^bsup>\<ge> Suc n\<^esup>\<close> by simp
+                 \<union> \<lbrakk> K\<^sub>1 \<Up> n \<rbrakk>\<^sub>p\<^sub>r\<^sub>i\<^sub>m \<inter> \<lbrakk> K\<^sub>2 \<not>\<Up> \<ge> n \<rbrakk>\<^sub>p\<^sub>r\<^sub>i\<^sub>m
+                 \<inter> \<lbrakk> K\<^sub>1 kills K\<^sub>2 \<rbrakk>\<^sub>T\<^sub>E\<^sub>S\<^sub>L\<^bsup>\<ge> Suc n\<^esup>\<close> by simp
   finally show ?thesis by blast
 qed
 
-fun TESL_interpretation_stepwise :: \<open>'\<tau>::linordered_field TESL_formula \<Rightarrow> nat \<Rightarrow> '\<tau> run set\<close> ("\<lbrakk>\<lbrakk> _ \<rbrakk>\<rbrakk>\<^sub>T\<^sub>E\<^sub>S\<^sub>L\<^bsup>\<ge> _\<^esup>") where
-    \<open>\<lbrakk>\<lbrakk> [] \<rbrakk>\<rbrakk>\<^sub>T\<^sub>E\<^sub>S\<^sub>L\<^bsup>\<ge> n\<^esup> = { _. True }\<close>
-  | \<open>\<lbrakk>\<lbrakk> \<phi> # \<Phi> \<rbrakk>\<rbrakk>\<^sub>T\<^sub>E\<^sub>S\<^sub>L\<^bsup>\<ge> n\<^esup> = \<lbrakk> \<phi> \<rbrakk>\<^sub>T\<^sub>E\<^sub>S\<^sub>L\<^bsup>\<ge> n\<^esup> \<inter> \<lbrakk>\<lbrakk> \<Phi> \<rbrakk>\<rbrakk>\<^sub>T\<^sub>E\<^sub>S\<^sub>L\<^bsup>\<ge> n\<^esup>\<close>
+fun TESL_interpretation_stepwise
+  ::\<open>'\<tau>::linordered_field TESL_formula \<Rightarrow> nat \<Rightarrow> '\<tau> run set\<close>
+  ("\<lbrakk>\<lbrakk> _ \<rbrakk>\<rbrakk>\<^sub>T\<^sub>E\<^sub>S\<^sub>L\<^bsup>\<ge> _\<^esup>")
+where
+  \<open>\<lbrakk>\<lbrakk> [] \<rbrakk>\<rbrakk>\<^sub>T\<^sub>E\<^sub>S\<^sub>L\<^bsup>\<ge> n\<^esup> = {\<rho>. True}\<close>
+| \<open>\<lbrakk>\<lbrakk> \<phi> # \<Phi> \<rbrakk>\<rbrakk>\<^sub>T\<^sub>E\<^sub>S\<^sub>L\<^bsup>\<ge> n\<^esup> = \<lbrakk> \<phi> \<rbrakk>\<^sub>T\<^sub>E\<^sub>S\<^sub>L\<^bsup>\<ge> n\<^esup> \<inter> \<lbrakk>\<lbrakk> \<Phi> \<rbrakk>\<rbrakk>\<^sub>T\<^sub>E\<^sub>S\<^sub>L\<^bsup>\<ge> n\<^esup>\<close>
 
 lemma TESL_interpretation_stepwise_fixpoint:
   \<open>\<lbrakk>\<lbrakk> \<Phi> \<rbrakk>\<rbrakk>\<^sub>T\<^sub>E\<^sub>S\<^sub>L\<^bsup>\<ge> n\<^esup> = \<Inter> ((\<lambda>\<phi>. \<lbrakk> \<phi> \<rbrakk>\<^sub>T\<^sub>E\<^sub>S\<^sub>L\<^bsup>\<ge> n\<^esup>) ` set \<Phi>)\<close>
@@ -323,21 +340,25 @@ by (induction \<Phi>\<^sub>1, simp, auto)
 
 section \<open>Interpretation of configurations\<close>
 
-fun HeronConf_interpretation :: \<open>'\<tau>::linordered_field config \<Rightarrow> '\<tau> run set\<close> ("\<lbrakk> _ \<rbrakk>\<^sub>c\<^sub>o\<^sub>n\<^sub>f\<^sub>i\<^sub>g" 71) where
+fun HeronConf_interpretation
+  ::\<open>'\<tau>::linordered_field config \<Rightarrow> '\<tau> run set\<close>          ("\<lbrakk> _ \<rbrakk>\<^sub>c\<^sub>o\<^sub>n\<^sub>f\<^sub>i\<^sub>g" 71)
+where
   \<open>\<lbrakk> \<Gamma>, n \<turnstile> \<Psi> \<triangleright> \<Phi> \<rbrakk>\<^sub>c\<^sub>o\<^sub>n\<^sub>f\<^sub>i\<^sub>g = \<lbrakk>\<lbrakk> \<Gamma> \<rbrakk>\<rbrakk>\<^sub>p\<^sub>r\<^sub>i\<^sub>m \<inter> \<lbrakk>\<lbrakk> \<Psi> \<rbrakk>\<rbrakk>\<^sub>T\<^sub>E\<^sub>S\<^sub>L\<^bsup>\<ge> n\<^esup> \<inter> \<lbrakk>\<lbrakk> \<Phi> \<rbrakk>\<rbrakk>\<^sub>T\<^sub>E\<^sub>S\<^sub>L\<^bsup>\<ge> Suc n\<^esup>\<close>
 
 lemma HeronConf_interp_composition:
-  shows \<open>\<lbrakk> \<Gamma>\<^sub>1, n \<turnstile> \<Psi>\<^sub>1 \<triangleright> \<Phi>\<^sub>1 \<rbrakk>\<^sub>c\<^sub>o\<^sub>n\<^sub>f\<^sub>i\<^sub>g \<inter> \<lbrakk> \<Gamma>\<^sub>2, n \<turnstile> \<Psi>\<^sub>2 \<triangleright> \<Phi>\<^sub>2 \<rbrakk>\<^sub>c\<^sub>o\<^sub>n\<^sub>f\<^sub>i\<^sub>g
-         = \<lbrakk> (\<Gamma>\<^sub>1 @ \<Gamma>\<^sub>2), n \<turnstile> (\<Psi>\<^sub>1 @ \<Psi>\<^sub>2) \<triangleright> (\<Phi>\<^sub>1 @ \<Phi>\<^sub>2) \<rbrakk>\<^sub>c\<^sub>o\<^sub>n\<^sub>f\<^sub>i\<^sub>g\<close>
+   \<open>\<lbrakk> \<Gamma>\<^sub>1, n \<turnstile> \<Psi>\<^sub>1 \<triangleright> \<Phi>\<^sub>1 \<rbrakk>\<^sub>c\<^sub>o\<^sub>n\<^sub>f\<^sub>i\<^sub>g \<inter> \<lbrakk> \<Gamma>\<^sub>2, n \<turnstile> \<Psi>\<^sub>2 \<triangleright> \<Phi>\<^sub>2 \<rbrakk>\<^sub>c\<^sub>o\<^sub>n\<^sub>f\<^sub>i\<^sub>g
+     = \<lbrakk> (\<Gamma>\<^sub>1 @ \<Gamma>\<^sub>2), n \<turnstile> (\<Psi>\<^sub>1 @ \<Psi>\<^sub>2) \<triangleright> (\<Phi>\<^sub>1 @ \<Phi>\<^sub>2) \<rbrakk>\<^sub>c\<^sub>o\<^sub>n\<^sub>f\<^sub>i\<^sub>g\<close>
   using TESL_interp_stepwise_composition symrun_interp_expansion
-  by (simp add: TESL_interp_stepwise_composition symrun_interp_expansion inf_assoc inf_left_commute)
+by (simp add: TESL_interp_stepwise_composition
+              symrun_interp_expansion inf_assoc inf_left_commute)
 
 lemma HeronConf_interp_stepwise_instant_cases:
-  shows \<open>\<lbrakk> \<Gamma>, n \<turnstile> [] \<triangleright> \<Phi> \<rbrakk>\<^sub>c\<^sub>o\<^sub>n\<^sub>f\<^sub>i\<^sub>g = \<lbrakk> \<Gamma>, Suc n \<turnstile> \<Phi> \<triangleright> [] \<rbrakk>\<^sub>c\<^sub>o\<^sub>n\<^sub>f\<^sub>i\<^sub>g\<close>
+   \<open>\<lbrakk> \<Gamma>, n \<turnstile> [] \<triangleright> \<Phi> \<rbrakk>\<^sub>c\<^sub>o\<^sub>n\<^sub>f\<^sub>i\<^sub>g = \<lbrakk> \<Gamma>, Suc n \<turnstile> \<Phi> \<triangleright> [] \<rbrakk>\<^sub>c\<^sub>o\<^sub>n\<^sub>f\<^sub>i\<^sub>g\<close>
 proof -
   have \<open>\<lbrakk> \<Gamma>, n \<turnstile> [] \<triangleright> \<Phi> \<rbrakk>\<^sub>c\<^sub>o\<^sub>n\<^sub>f\<^sub>i\<^sub>g = \<lbrakk>\<lbrakk> \<Gamma> \<rbrakk>\<rbrakk>\<^sub>p\<^sub>r\<^sub>i\<^sub>m \<inter> \<lbrakk>\<lbrakk> [] \<rbrakk>\<rbrakk>\<^sub>T\<^sub>E\<^sub>S\<^sub>L\<^bsup>\<ge> n\<^esup> \<inter> \<lbrakk>\<lbrakk> \<Phi> \<rbrakk>\<rbrakk>\<^sub>T\<^sub>E\<^sub>S\<^sub>L\<^bsup>\<ge> Suc n\<^esup>\<close>
     by simp
-  moreover have \<open>\<lbrakk> \<Gamma>, Suc n \<turnstile> \<Phi> \<triangleright> [] \<rbrakk>\<^sub>c\<^sub>o\<^sub>n\<^sub>f\<^sub>i\<^sub>g = \<lbrakk>\<lbrakk> \<Gamma> \<rbrakk>\<rbrakk>\<^sub>p\<^sub>r\<^sub>i\<^sub>m \<inter> \<lbrakk>\<lbrakk> \<Phi> \<rbrakk>\<rbrakk>\<^sub>T\<^sub>E\<^sub>S\<^sub>L\<^bsup>\<ge> Suc n\<^esup> \<inter> \<lbrakk>\<lbrakk> [] \<rbrakk>\<rbrakk>\<^sub>T\<^sub>E\<^sub>S\<^sub>L\<^bsup>\<ge> Suc n\<^esup>\<close>
+  moreover have \<open>\<lbrakk> \<Gamma>, Suc n \<turnstile> \<Phi> \<triangleright> [] \<rbrakk>\<^sub>c\<^sub>o\<^sub>n\<^sub>f\<^sub>i\<^sub>g
+                  = \<lbrakk>\<lbrakk> \<Gamma> \<rbrakk>\<rbrakk>\<^sub>p\<^sub>r\<^sub>i\<^sub>m \<inter> \<lbrakk>\<lbrakk> \<Phi> \<rbrakk>\<rbrakk>\<^sub>T\<^sub>E\<^sub>S\<^sub>L\<^bsup>\<ge> Suc n\<^esup> \<inter> \<lbrakk>\<lbrakk> [] \<rbrakk>\<rbrakk>\<^sub>T\<^sub>E\<^sub>S\<^sub>L\<^bsup>\<ge> Suc n\<^esup>\<close>
     by simp
   moreover have \<open>\<lbrakk>\<lbrakk> \<Gamma> \<rbrakk>\<rbrakk>\<^sub>p\<^sub>r\<^sub>i\<^sub>m \<inter> \<lbrakk>\<lbrakk> [] \<rbrakk>\<rbrakk>\<^sub>T\<^sub>E\<^sub>S\<^sub>L\<^bsup>\<ge> n\<^esup> \<inter> \<lbrakk>\<lbrakk> \<Phi> \<rbrakk>\<rbrakk>\<^sub>T\<^sub>E\<^sub>S\<^sub>L\<^bsup>\<ge> Suc n\<^esup>
                  = \<lbrakk>\<lbrakk> \<Gamma> \<rbrakk>\<rbrakk>\<^sub>p\<^sub>r\<^sub>i\<^sub>m \<inter> \<lbrakk>\<lbrakk> \<Phi> \<rbrakk>\<rbrakk>\<^sub>T\<^sub>E\<^sub>S\<^sub>L\<^bsup>\<ge> Suc n\<^esup> \<inter> \<lbrakk>\<lbrakk> [] \<rbrakk>\<rbrakk>\<^sub>T\<^sub>E\<^sub>S\<^sub>L\<^bsup>\<ge> Suc n\<^esup>\<close>
@@ -346,121 +367,162 @@ proof -
 qed
 
 lemma HeronConf_interp_stepwise_sporadicon_cases:
-  shows \<open>\<lbrakk> \<Gamma>, n \<turnstile> ((K\<^sub>1 sporadic \<tau> on K\<^sub>2) # \<Psi>) \<triangleright> \<Phi> \<rbrakk>\<^sub>c\<^sub>o\<^sub>n\<^sub>f\<^sub>i\<^sub>g
-          = \<lbrakk> \<Gamma>, n \<turnstile> \<Psi> \<triangleright> ((K\<^sub>1 sporadic \<tau> on K\<^sub>2) # \<Phi>) \<rbrakk>\<^sub>c\<^sub>o\<^sub>n\<^sub>f\<^sub>i\<^sub>g
-          \<union> \<lbrakk> ((K\<^sub>1 \<Up> n) # (K\<^sub>2 \<Down> n @ \<tau>) # \<Gamma>), n \<turnstile> \<Psi> \<triangleright> \<Phi> \<rbrakk>\<^sub>c\<^sub>o\<^sub>n\<^sub>f\<^sub>i\<^sub>g\<close>
+   \<open>\<lbrakk> \<Gamma>, n \<turnstile> ((K\<^sub>1 sporadic \<tau> on K\<^sub>2) # \<Psi>) \<triangleright> \<Phi> \<rbrakk>\<^sub>c\<^sub>o\<^sub>n\<^sub>f\<^sub>i\<^sub>g
+    = \<lbrakk> \<Gamma>, n \<turnstile> \<Psi> \<triangleright> ((K\<^sub>1 sporadic \<tau> on K\<^sub>2) # \<Phi>) \<rbrakk>\<^sub>c\<^sub>o\<^sub>n\<^sub>f\<^sub>i\<^sub>g
+    \<union> \<lbrakk> ((K\<^sub>1 \<Up> n) # (K\<^sub>2 \<Down> n @ \<tau>) # \<Gamma>), n \<turnstile> \<Psi> \<triangleright> \<Phi> \<rbrakk>\<^sub>c\<^sub>o\<^sub>n\<^sub>f\<^sub>i\<^sub>g\<close>
 proof -
-  have \<open>\<lbrakk> \<Gamma>, n \<turnstile> (K\<^sub>1 sporadic \<tau> on K\<^sub>2) # \<Psi> \<triangleright> \<Phi> \<rbrakk>\<^sub>c\<^sub>o\<^sub>n\<^sub>f\<^sub>i\<^sub>g = \<lbrakk>\<lbrakk> \<Gamma> \<rbrakk>\<rbrakk>\<^sub>p\<^sub>r\<^sub>i\<^sub>m \<inter> \<lbrakk>\<lbrakk> (K\<^sub>1 sporadic \<tau> on K\<^sub>2) # \<Psi> \<rbrakk>\<rbrakk>\<^sub>T\<^sub>E\<^sub>S\<^sub>L\<^bsup>\<ge> n\<^esup> \<inter> \<lbrakk>\<lbrakk> \<Phi> \<rbrakk>\<rbrakk>\<^sub>T\<^sub>E\<^sub>S\<^sub>L\<^bsup>\<ge> Suc n\<^esup>\<close>
+  have \<open>\<lbrakk> \<Gamma>, n \<turnstile> (K\<^sub>1 sporadic \<tau> on K\<^sub>2) # \<Psi> \<triangleright> \<Phi> \<rbrakk>\<^sub>c\<^sub>o\<^sub>n\<^sub>f\<^sub>i\<^sub>g
+        = \<lbrakk>\<lbrakk> \<Gamma> \<rbrakk>\<rbrakk>\<^sub>p\<^sub>r\<^sub>i\<^sub>m \<inter> \<lbrakk>\<lbrakk> (K\<^sub>1 sporadic \<tau> on K\<^sub>2) # \<Psi> \<rbrakk>\<rbrakk>\<^sub>T\<^sub>E\<^sub>S\<^sub>L\<^bsup>\<ge> n\<^esup> \<inter> \<lbrakk>\<lbrakk> \<Phi> \<rbrakk>\<rbrakk>\<^sub>T\<^sub>E\<^sub>S\<^sub>L\<^bsup>\<ge> Suc n\<^esup>\<close>
     by simp
-  moreover have \<open>\<lbrakk> \<Gamma>, n \<turnstile> \<Psi> \<triangleright> ((K\<^sub>1 sporadic \<tau> on K\<^sub>2) # \<Phi>) \<rbrakk>\<^sub>c\<^sub>o\<^sub>n\<^sub>f\<^sub>i\<^sub>g = \<lbrakk>\<lbrakk> \<Gamma> \<rbrakk>\<rbrakk>\<^sub>p\<^sub>r\<^sub>i\<^sub>m \<inter> \<lbrakk>\<lbrakk> \<Psi> \<rbrakk>\<rbrakk>\<^sub>T\<^sub>E\<^sub>S\<^sub>L\<^bsup>\<ge> n\<^esup> \<inter> \<lbrakk>\<lbrakk> (K\<^sub>1 sporadic \<tau> on K\<^sub>2) # \<Phi> \<rbrakk>\<rbrakk>\<^sub>T\<^sub>E\<^sub>S\<^sub>L\<^bsup>\<ge> Suc n\<^esup>\<close>
+  moreover have \<open>\<lbrakk> \<Gamma>, n \<turnstile> \<Psi> \<triangleright> ((K\<^sub>1 sporadic \<tau> on K\<^sub>2) # \<Phi>) \<rbrakk>\<^sub>c\<^sub>o\<^sub>n\<^sub>f\<^sub>i\<^sub>g
+                 =  \<lbrakk>\<lbrakk> \<Gamma> \<rbrakk>\<rbrakk>\<^sub>p\<^sub>r\<^sub>i\<^sub>m \<inter> \<lbrakk>\<lbrakk> \<Psi> \<rbrakk>\<rbrakk>\<^sub>T\<^sub>E\<^sub>S\<^sub>L\<^bsup>\<ge> n\<^esup>
+                  \<inter> \<lbrakk>\<lbrakk> (K\<^sub>1 sporadic \<tau> on K\<^sub>2) # \<Phi> \<rbrakk>\<rbrakk>\<^sub>T\<^sub>E\<^sub>S\<^sub>L\<^bsup>\<ge> Suc n\<^esup>\<close>
     by simp
-  moreover have \<open>\<lbrakk> ((K\<^sub>1 \<Up> n) # (K\<^sub>2 \<Down> n @ \<tau>) # \<Gamma>), n \<turnstile> \<Psi> \<triangleright> \<Phi> \<rbrakk>\<^sub>c\<^sub>o\<^sub>n\<^sub>f\<^sub>i\<^sub>g = \<lbrakk>\<lbrakk> ((K\<^sub>1 \<Up> n) # (K\<^sub>2 \<Down> n @ \<tau>) # \<Gamma>) \<rbrakk>\<rbrakk>\<^sub>p\<^sub>r\<^sub>i\<^sub>m \<inter> \<lbrakk>\<lbrakk> \<Psi> \<rbrakk>\<rbrakk>\<^sub>T\<^sub>E\<^sub>S\<^sub>L\<^bsup>\<ge> n\<^esup> \<inter> \<lbrakk>\<lbrakk> \<Phi> \<rbrakk>\<rbrakk>\<^sub>T\<^sub>E\<^sub>S\<^sub>L\<^bsup>\<ge> Suc n\<^esup>\<close>
+  moreover have \<open>\<lbrakk> ((K\<^sub>1 \<Up> n) # (K\<^sub>2 \<Down> n @ \<tau>) # \<Gamma>), n \<turnstile> \<Psi> \<triangleright> \<Phi> \<rbrakk>\<^sub>c\<^sub>o\<^sub>n\<^sub>f\<^sub>i\<^sub>g
+                 =  \<lbrakk>\<lbrakk> ((K\<^sub>1 \<Up> n) # (K\<^sub>2 \<Down> n @ \<tau>) # \<Gamma>) \<rbrakk>\<rbrakk>\<^sub>p\<^sub>r\<^sub>i\<^sub>m
+                  \<inter> \<lbrakk>\<lbrakk> \<Psi> \<rbrakk>\<rbrakk>\<^sub>T\<^sub>E\<^sub>S\<^sub>L\<^bsup>\<ge> n\<^esup> \<inter> \<lbrakk>\<lbrakk> \<Phi> \<rbrakk>\<rbrakk>\<^sub>T\<^sub>E\<^sub>S\<^sub>L\<^bsup>\<ge> Suc n\<^esup>\<close>
     by simp
   ultimately show ?thesis
   proof -
-    have \<open>(\<lbrakk> K\<^sub>1 \<Up> n \<rbrakk>\<^sub>p\<^sub>r\<^sub>i\<^sub>m \<inter> \<lbrakk> K\<^sub>2 \<Down> n @ \<tau> \<rbrakk>\<^sub>p\<^sub>r\<^sub>i\<^sub>m \<union> \<lbrakk> K\<^sub>1 sporadic \<tau> on K\<^sub>2 \<rbrakk>\<^sub>T\<^sub>E\<^sub>S\<^sub>L\<^bsup>\<ge> Suc n\<^esup>) \<inter> (\<lbrakk>\<lbrakk> \<Gamma> \<rbrakk>\<rbrakk>\<^sub>p\<^sub>r\<^sub>i\<^sub>m \<inter> \<lbrakk>\<lbrakk> \<Psi> \<rbrakk>\<rbrakk>\<^sub>T\<^sub>E\<^sub>S\<^sub>L\<^bsup>\<ge> n\<^esup>) = \<lbrakk> K\<^sub>1 sporadic \<tau> on K\<^sub>2 \<rbrakk>\<^sub>T\<^sub>E\<^sub>S\<^sub>L\<^bsup>\<ge> n\<^esup> \<inter> (\<lbrakk>\<lbrakk> \<Psi> \<rbrakk>\<rbrakk>\<^sub>T\<^sub>E\<^sub>S\<^sub>L\<^bsup>\<ge> n\<^esup> \<inter> \<lbrakk>\<lbrakk> \<Gamma> \<rbrakk>\<rbrakk>\<^sub>p\<^sub>r\<^sub>i\<^sub>m)\<close>
+    have \<open>(\<lbrakk> K\<^sub>1 \<Up> n \<rbrakk>\<^sub>p\<^sub>r\<^sub>i\<^sub>m \<inter> \<lbrakk> K\<^sub>2 \<Down> n @ \<tau> \<rbrakk>\<^sub>p\<^sub>r\<^sub>i\<^sub>m \<union> \<lbrakk> K\<^sub>1 sporadic \<tau> on K\<^sub>2 \<rbrakk>\<^sub>T\<^sub>E\<^sub>S\<^sub>L\<^bsup>\<ge> Suc n\<^esup>)
+            \<inter> (\<lbrakk>\<lbrakk> \<Gamma> \<rbrakk>\<rbrakk>\<^sub>p\<^sub>r\<^sub>i\<^sub>m \<inter> \<lbrakk>\<lbrakk> \<Psi> \<rbrakk>\<rbrakk>\<^sub>T\<^sub>E\<^sub>S\<^sub>L\<^bsup>\<ge> n\<^esup>)
+          = \<lbrakk> K\<^sub>1 sporadic \<tau> on K\<^sub>2 \<rbrakk>\<^sub>T\<^sub>E\<^sub>S\<^sub>L\<^bsup>\<ge> n\<^esup> \<inter> (\<lbrakk>\<lbrakk> \<Psi> \<rbrakk>\<rbrakk>\<^sub>T\<^sub>E\<^sub>S\<^sub>L\<^bsup>\<ge> n\<^esup> \<inter> \<lbrakk>\<lbrakk> \<Gamma> \<rbrakk>\<rbrakk>\<^sub>p\<^sub>r\<^sub>i\<^sub>m)\<close>
       using TESL_interp_stepwise_sporadicon_coind_unfold by blast
-    then have \<open>\<lbrakk>\<lbrakk> ((K\<^sub>1 \<Up> n) # (K\<^sub>2 \<Down> n @ \<tau>) # \<Gamma>) \<rbrakk>\<rbrakk>\<^sub>p\<^sub>r\<^sub>i\<^sub>m \<inter> \<lbrakk>\<lbrakk> \<Psi> \<rbrakk>\<rbrakk>\<^sub>T\<^sub>E\<^sub>S\<^sub>L\<^bsup>\<ge> n\<^esup> \<union> \<lbrakk>\<lbrakk> \<Gamma> \<rbrakk>\<rbrakk>\<^sub>p\<^sub>r\<^sub>i\<^sub>m \<inter> \<lbrakk>\<lbrakk> \<Psi> \<rbrakk>\<rbrakk>\<^sub>T\<^sub>E\<^sub>S\<^sub>L\<^bsup>\<ge> n\<^esup> \<inter> \<lbrakk> K\<^sub>1 sporadic \<tau> on K\<^sub>2 \<rbrakk>\<^sub>T\<^sub>E\<^sub>S\<^sub>L\<^bsup>\<ge> Suc n\<^esup> = \<lbrakk>\<lbrakk> (K\<^sub>1 sporadic \<tau> on K\<^sub>2) # \<Psi> \<rbrakk>\<rbrakk>\<^sub>T\<^sub>E\<^sub>S\<^sub>L\<^bsup>\<ge> n\<^esup> \<inter> \<lbrakk>\<lbrakk> \<Gamma> \<rbrakk>\<rbrakk>\<^sub>p\<^sub>r\<^sub>i\<^sub>m\<close>
-      by auto
-    then show ?thesis
-      by auto
+    hence \<open>\<lbrakk>\<lbrakk> ((K\<^sub>1 \<Up> n) # (K\<^sub>2 \<Down> n @ \<tau>) # \<Gamma>) \<rbrakk>\<rbrakk>\<^sub>p\<^sub>r\<^sub>i\<^sub>m \<inter> \<lbrakk>\<lbrakk> \<Psi> \<rbrakk>\<rbrakk>\<^sub>T\<^sub>E\<^sub>S\<^sub>L\<^bsup>\<ge> n\<^esup>
+            \<union> \<lbrakk>\<lbrakk> \<Gamma> \<rbrakk>\<rbrakk>\<^sub>p\<^sub>r\<^sub>i\<^sub>m \<inter> \<lbrakk>\<lbrakk> \<Psi> \<rbrakk>\<rbrakk>\<^sub>T\<^sub>E\<^sub>S\<^sub>L\<^bsup>\<ge> n\<^esup> \<inter> \<lbrakk> K\<^sub>1 sporadic \<tau> on K\<^sub>2 \<rbrakk>\<^sub>T\<^sub>E\<^sub>S\<^sub>L\<^bsup>\<ge> Suc n\<^esup>
+           = \<lbrakk>\<lbrakk> (K\<^sub>1 sporadic \<tau> on K\<^sub>2) # \<Psi> \<rbrakk>\<rbrakk>\<^sub>T\<^sub>E\<^sub>S\<^sub>L\<^bsup>\<ge> n\<^esup> \<inter> \<lbrakk>\<lbrakk> \<Gamma> \<rbrakk>\<rbrakk>\<^sub>p\<^sub>r\<^sub>i\<^sub>m\<close> by auto
+    thus ?thesis by auto
   qed
 qed
 
 lemma HeronConf_interp_stepwise_tagrel_cases:
-  shows \<open>\<lbrakk> \<Gamma>, n \<turnstile> ((time-relation \<lfloor>K\<^sub>1, K\<^sub>2\<rfloor> \<in> R) # \<Psi>) \<triangleright> \<Phi> \<rbrakk>\<^sub>c\<^sub>o\<^sub>n\<^sub>f\<^sub>i\<^sub>g
-          = \<lbrakk> ((\<lfloor>\<tau>\<^sub>v\<^sub>a\<^sub>r(K\<^sub>1, n), \<tau>\<^sub>v\<^sub>a\<^sub>r(K\<^sub>2, n)\<rfloor> \<in> R) # \<Gamma>), n \<turnstile> \<Psi> \<triangleright> ((time-relation \<lfloor>K\<^sub>1, K\<^sub>2\<rfloor> \<in> R) # \<Phi>) \<rbrakk>\<^sub>c\<^sub>o\<^sub>n\<^sub>f\<^sub>i\<^sub>g\<close>
+   \<open>\<lbrakk> \<Gamma>, n \<turnstile> ((time-relation \<lfloor>K\<^sub>1, K\<^sub>2\<rfloor> \<in> R) # \<Psi>) \<triangleright> \<Phi> \<rbrakk>\<^sub>c\<^sub>o\<^sub>n\<^sub>f\<^sub>i\<^sub>g
+    = \<lbrakk> ((\<lfloor>\<tau>\<^sub>v\<^sub>a\<^sub>r(K\<^sub>1, n), \<tau>\<^sub>v\<^sub>a\<^sub>r(K\<^sub>2, n)\<rfloor> \<in> R) # \<Gamma>), n
+        \<turnstile> \<Psi> \<triangleright> ((time-relation \<lfloor>K\<^sub>1, K\<^sub>2\<rfloor> \<in> R) # \<Phi>) \<rbrakk>\<^sub>c\<^sub>o\<^sub>n\<^sub>f\<^sub>i\<^sub>g\<close>
 proof -
-  have \<open>\<lbrakk> \<Gamma>, n \<turnstile> (time-relation \<lfloor>K\<^sub>1, K\<^sub>2\<rfloor> \<in> R) # \<Psi> \<triangleright> \<Phi> \<rbrakk>\<^sub>c\<^sub>o\<^sub>n\<^sub>f\<^sub>i\<^sub>g = \<lbrakk>\<lbrakk> \<Gamma> \<rbrakk>\<rbrakk>\<^sub>p\<^sub>r\<^sub>i\<^sub>m \<inter> \<lbrakk>\<lbrakk> (time-relation \<lfloor>K\<^sub>1, K\<^sub>2\<rfloor> \<in> R) # \<Psi> \<rbrakk>\<rbrakk>\<^sub>T\<^sub>E\<^sub>S\<^sub>L\<^bsup>\<ge> n\<^esup> \<inter> \<lbrakk>\<lbrakk> \<Phi> \<rbrakk>\<rbrakk>\<^sub>T\<^sub>E\<^sub>S\<^sub>L\<^bsup>\<ge> Suc n\<^esup>\<close>
-    by simp
-  moreover have \<open>\<lbrakk> ((\<lfloor>\<tau>\<^sub>v\<^sub>a\<^sub>r(K\<^sub>1, n), \<tau>\<^sub>v\<^sub>a\<^sub>r(K\<^sub>2, n)\<rfloor> \<in> R) # \<Gamma>), n \<turnstile> \<Psi> \<triangleright> ((time-relation \<lfloor>K\<^sub>1, K\<^sub>2\<rfloor> \<in> R) # \<Phi>) \<rbrakk>\<^sub>c\<^sub>o\<^sub>n\<^sub>f\<^sub>i\<^sub>g
-                    = \<lbrakk>\<lbrakk> (\<lfloor>\<tau>\<^sub>v\<^sub>a\<^sub>r(K\<^sub>1, n), \<tau>\<^sub>v\<^sub>a\<^sub>r(K\<^sub>2, n)\<rfloor> \<in> R) # \<Gamma> \<rbrakk>\<rbrakk>\<^sub>p\<^sub>r\<^sub>i\<^sub>m \<inter> \<lbrakk>\<lbrakk> \<Psi> \<rbrakk>\<rbrakk>\<^sub>T\<^sub>E\<^sub>S\<^sub>L\<^bsup>\<ge> n\<^esup> \<inter> \<lbrakk>\<lbrakk> (time-relation \<lfloor>K\<^sub>1, K\<^sub>2\<rfloor> \<in> R) # \<Phi> \<rbrakk>\<rbrakk>\<^sub>T\<^sub>E\<^sub>S\<^sub>L\<^bsup>\<ge> Suc n\<^esup>\<close>
+  have \<open>\<lbrakk> \<Gamma>, n \<turnstile> (time-relation \<lfloor>K\<^sub>1, K\<^sub>2\<rfloor> \<in> R) # \<Psi> \<triangleright> \<Phi> \<rbrakk>\<^sub>c\<^sub>o\<^sub>n\<^sub>f\<^sub>i\<^sub>g
+        = \<lbrakk>\<lbrakk> \<Gamma> \<rbrakk>\<rbrakk>\<^sub>p\<^sub>r\<^sub>i\<^sub>m \<inter> \<lbrakk>\<lbrakk> (time-relation \<lfloor>K\<^sub>1, K\<^sub>2\<rfloor> \<in> R) # \<Psi> \<rbrakk>\<rbrakk>\<^sub>T\<^sub>E\<^sub>S\<^sub>L\<^bsup>\<ge> n\<^esup>
+        \<inter> \<lbrakk>\<lbrakk> \<Phi> \<rbrakk>\<rbrakk>\<^sub>T\<^sub>E\<^sub>S\<^sub>L\<^bsup>\<ge> Suc n\<^esup>\<close> by simp
+  moreover have \<open>\<lbrakk> ((\<lfloor>\<tau>\<^sub>v\<^sub>a\<^sub>r(K\<^sub>1, n), \<tau>\<^sub>v\<^sub>a\<^sub>r(K\<^sub>2, n)\<rfloor> \<in> R) # \<Gamma>), n
+                  \<turnstile> \<Psi> \<triangleright> ((time-relation \<lfloor>K\<^sub>1, K\<^sub>2\<rfloor> \<in> R) # \<Phi>) \<rbrakk>\<^sub>c\<^sub>o\<^sub>n\<^sub>f\<^sub>i\<^sub>g
+                 = \<lbrakk>\<lbrakk> (\<lfloor>\<tau>\<^sub>v\<^sub>a\<^sub>r(K\<^sub>1, n), \<tau>\<^sub>v\<^sub>a\<^sub>r(K\<^sub>2, n)\<rfloor> \<in> R) # \<Gamma> \<rbrakk>\<rbrakk>\<^sub>p\<^sub>r\<^sub>i\<^sub>m \<inter> \<lbrakk>\<lbrakk> \<Psi> \<rbrakk>\<rbrakk>\<^sub>T\<^sub>E\<^sub>S\<^sub>L\<^bsup>\<ge> n\<^esup>
+                 \<inter> \<lbrakk>\<lbrakk> (time-relation \<lfloor>K\<^sub>1, K\<^sub>2\<rfloor> \<in> R) # \<Phi> \<rbrakk>\<rbrakk>\<^sub>T\<^sub>E\<^sub>S\<^sub>L\<^bsup>\<ge> Suc n\<^esup>\<close>
     by simp
   ultimately show ?thesis
   proof -
-    have \<open>\<lbrakk> \<lfloor>\<tau>\<^sub>v\<^sub>a\<^sub>r(K\<^sub>1, n), \<tau>\<^sub>v\<^sub>a\<^sub>r(K\<^sub>2, n)\<rfloor> \<in> R \<rbrakk>\<^sub>p\<^sub>r\<^sub>i\<^sub>m \<inter> \<lbrakk> time-relation \<lfloor>K\<^sub>1, K\<^sub>2\<rfloor> \<in> R \<rbrakk>\<^sub>T\<^sub>E\<^sub>S\<^sub>L\<^bsup>\<ge> Suc n\<^esup> \<inter> \<lbrakk>\<lbrakk> \<Psi> \<rbrakk>\<rbrakk>\<^sub>T\<^sub>E\<^sub>S\<^sub>L\<^bsup>\<ge> n\<^esup> = \<lbrakk>\<lbrakk> (time-relation \<lfloor>K\<^sub>1, K\<^sub>2\<rfloor> \<in> R) # \<Psi> \<rbrakk>\<rbrakk>\<^sub>T\<^sub>E\<^sub>S\<^sub>L\<^bsup>\<ge> n\<^esup>\<close>
-      using TESL_interp_stepwise_tagrel_coind_unfold TESL_interpretation_stepwise_cons_morph by blast
-    then show ?thesis
-      by auto
+    have \<open>\<lbrakk> \<lfloor>\<tau>\<^sub>v\<^sub>a\<^sub>r(K\<^sub>1, n), \<tau>\<^sub>v\<^sub>a\<^sub>r(K\<^sub>2, n)\<rfloor> \<in> R \<rbrakk>\<^sub>p\<^sub>r\<^sub>i\<^sub>m
+          \<inter> \<lbrakk> time-relation \<lfloor>K\<^sub>1, K\<^sub>2\<rfloor> \<in> R \<rbrakk>\<^sub>T\<^sub>E\<^sub>S\<^sub>L\<^bsup>\<ge> Suc n\<^esup>
+          \<inter> \<lbrakk>\<lbrakk> \<Psi> \<rbrakk>\<rbrakk>\<^sub>T\<^sub>E\<^sub>S\<^sub>L\<^bsup>\<ge> n\<^esup> = \<lbrakk>\<lbrakk> (time-relation \<lfloor>K\<^sub>1, K\<^sub>2\<rfloor> \<in> R) # \<Psi> \<rbrakk>\<rbrakk>\<^sub>T\<^sub>E\<^sub>S\<^sub>L\<^bsup>\<ge> n\<^esup>\<close>
+      using TESL_interp_stepwise_tagrel_coind_unfold
+            TESL_interpretation_stepwise_cons_morph by blast
+    thus ?thesis by auto
   qed
 qed
 
 lemma HeronConf_interp_stepwise_implies_cases:
-  shows \<open>\<lbrakk> \<Gamma>, n \<turnstile> ((K\<^sub>1 implies K\<^sub>2) # \<Psi>) \<triangleright> \<Phi> \<rbrakk>\<^sub>c\<^sub>o\<^sub>n\<^sub>f\<^sub>i\<^sub>g
-          = \<lbrakk> ((K\<^sub>1 \<not>\<Up> n) # \<Gamma>), n \<turnstile> \<Psi> \<triangleright> ((K\<^sub>1 implies K\<^sub>2) # \<Phi>) \<rbrakk>\<^sub>c\<^sub>o\<^sub>n\<^sub>f\<^sub>i\<^sub>g
-          \<union> \<lbrakk> ((K\<^sub>1 \<Up> n) # (K\<^sub>2 \<Up> n) # \<Gamma>), n \<turnstile> \<Psi> \<triangleright> ((K\<^sub>1 implies K\<^sub>2) # \<Phi>) \<rbrakk>\<^sub>c\<^sub>o\<^sub>n\<^sub>f\<^sub>i\<^sub>g\<close>
+   \<open>\<lbrakk> \<Gamma>, n \<turnstile> ((K\<^sub>1 implies K\<^sub>2) # \<Psi>) \<triangleright> \<Phi> \<rbrakk>\<^sub>c\<^sub>o\<^sub>n\<^sub>f\<^sub>i\<^sub>g
+      = \<lbrakk> ((K\<^sub>1 \<not>\<Up> n) # \<Gamma>), n \<turnstile> \<Psi> \<triangleright> ((K\<^sub>1 implies K\<^sub>2) # \<Phi>) \<rbrakk>\<^sub>c\<^sub>o\<^sub>n\<^sub>f\<^sub>i\<^sub>g
+      \<union> \<lbrakk> ((K\<^sub>1 \<Up> n) # (K\<^sub>2 \<Up> n) # \<Gamma>), n \<turnstile> \<Psi> \<triangleright> ((K\<^sub>1 implies K\<^sub>2) # \<Phi>) \<rbrakk>\<^sub>c\<^sub>o\<^sub>n\<^sub>f\<^sub>i\<^sub>g\<close>
 proof -
-  have \<open>\<lbrakk> \<Gamma>, n \<turnstile> (K\<^sub>1 implies K\<^sub>2) # \<Psi> \<triangleright> \<Phi> \<rbrakk>\<^sub>c\<^sub>o\<^sub>n\<^sub>f\<^sub>i\<^sub>g = \<lbrakk>\<lbrakk> \<Gamma> \<rbrakk>\<rbrakk>\<^sub>p\<^sub>r\<^sub>i\<^sub>m \<inter> \<lbrakk>\<lbrakk> (K\<^sub>1 implies K\<^sub>2) # \<Psi> \<rbrakk>\<rbrakk>\<^sub>T\<^sub>E\<^sub>S\<^sub>L\<^bsup>\<ge> n\<^esup> \<inter> \<lbrakk>\<lbrakk> \<Phi> \<rbrakk>\<rbrakk>\<^sub>T\<^sub>E\<^sub>S\<^sub>L\<^bsup>\<ge> Suc n\<^esup>\<close>
+  have \<open>\<lbrakk> \<Gamma>, n \<turnstile> (K\<^sub>1 implies K\<^sub>2) # \<Psi> \<triangleright> \<Phi> \<rbrakk>\<^sub>c\<^sub>o\<^sub>n\<^sub>f\<^sub>i\<^sub>g
+        = \<lbrakk>\<lbrakk> \<Gamma> \<rbrakk>\<rbrakk>\<^sub>p\<^sub>r\<^sub>i\<^sub>m \<inter> \<lbrakk>\<lbrakk> (K\<^sub>1 implies K\<^sub>2) # \<Psi> \<rbrakk>\<rbrakk>\<^sub>T\<^sub>E\<^sub>S\<^sub>L\<^bsup>\<ge> n\<^esup> \<inter> \<lbrakk>\<lbrakk> \<Phi> \<rbrakk>\<rbrakk>\<^sub>T\<^sub>E\<^sub>S\<^sub>L\<^bsup>\<ge> Suc n\<^esup>\<close>
     by simp
-  moreover have \<open>\<lbrakk> ((K\<^sub>1 \<not>\<Up> n) # \<Gamma>), n \<turnstile> \<Psi> \<triangleright> ((K\<^sub>1 implies K\<^sub>2) # \<Phi>) \<rbrakk>\<^sub>c\<^sub>o\<^sub>n\<^sub>f\<^sub>i\<^sub>g = \<lbrakk>\<lbrakk> (K\<^sub>1 \<not>\<Up> n) # \<Gamma> \<rbrakk>\<rbrakk>\<^sub>p\<^sub>r\<^sub>i\<^sub>m \<inter> \<lbrakk>\<lbrakk> \<Psi> \<rbrakk>\<rbrakk>\<^sub>T\<^sub>E\<^sub>S\<^sub>L\<^bsup>\<ge> n\<^esup> \<inter> \<lbrakk>\<lbrakk> (K\<^sub>1 implies K\<^sub>2) # \<Phi> \<rbrakk>\<rbrakk>\<^sub>T\<^sub>E\<^sub>S\<^sub>L\<^bsup>\<ge> Suc n\<^esup>\<close>
-    by simp
-  moreover have \<open>\<lbrakk> ((K\<^sub>1 \<Up> n) # (K\<^sub>2 \<Up> n) # \<Gamma>), n \<turnstile> \<Psi> \<triangleright> ((K\<^sub>1 implies K\<^sub>2) # \<Phi>) \<rbrakk>\<^sub>c\<^sub>o\<^sub>n\<^sub>f\<^sub>i\<^sub>g = \<lbrakk>\<lbrakk> ((K\<^sub>1 \<Up> n) # (K\<^sub>2 \<Up> n) # \<Gamma>) \<rbrakk>\<rbrakk>\<^sub>p\<^sub>r\<^sub>i\<^sub>m \<inter> \<lbrakk>\<lbrakk> \<Psi> \<rbrakk>\<rbrakk>\<^sub>T\<^sub>E\<^sub>S\<^sub>L\<^bsup>\<ge> n\<^esup> \<inter> \<lbrakk>\<lbrakk> (K\<^sub>1 implies K\<^sub>2) # \<Phi> \<rbrakk>\<rbrakk>\<^sub>T\<^sub>E\<^sub>S\<^sub>L\<^bsup>\<ge> Suc n\<^esup>\<close>
-    by simp
+  moreover have \<open>\<lbrakk> ((K\<^sub>1 \<not>\<Up> n) # \<Gamma>), n \<turnstile> \<Psi> \<triangleright> ((K\<^sub>1 implies K\<^sub>2) # \<Phi>) \<rbrakk>\<^sub>c\<^sub>o\<^sub>n\<^sub>f\<^sub>i\<^sub>g
+                = \<lbrakk>\<lbrakk> (K\<^sub>1 \<not>\<Up> n) # \<Gamma> \<rbrakk>\<rbrakk>\<^sub>p\<^sub>r\<^sub>i\<^sub>m \<inter> \<lbrakk>\<lbrakk> \<Psi> \<rbrakk>\<rbrakk>\<^sub>T\<^sub>E\<^sub>S\<^sub>L\<^bsup>\<ge> n\<^esup>
+                \<inter> \<lbrakk>\<lbrakk> (K\<^sub>1 implies K\<^sub>2) # \<Phi> \<rbrakk>\<rbrakk>\<^sub>T\<^sub>E\<^sub>S\<^sub>L\<^bsup>\<ge> Suc n\<^esup>\<close> by simp
+  moreover have \<open>\<lbrakk> ((K\<^sub>1 \<Up> n) # (K\<^sub>2 \<Up> n) # \<Gamma>), n \<turnstile> \<Psi> \<triangleright> ((K\<^sub>1 implies K\<^sub>2) # \<Phi>) \<rbrakk>\<^sub>c\<^sub>o\<^sub>n\<^sub>f\<^sub>i\<^sub>g
+                =  \<lbrakk>\<lbrakk> ((K\<^sub>1 \<Up> n) # (K\<^sub>2 \<Up> n) # \<Gamma>) \<rbrakk>\<rbrakk>\<^sub>p\<^sub>r\<^sub>i\<^sub>m \<inter> \<lbrakk>\<lbrakk> \<Psi> \<rbrakk>\<rbrakk>\<^sub>T\<^sub>E\<^sub>S\<^sub>L\<^bsup>\<ge> n\<^esup>
+                 \<inter> \<lbrakk>\<lbrakk> (K\<^sub>1 implies K\<^sub>2) # \<Phi> \<rbrakk>\<rbrakk>\<^sub>T\<^sub>E\<^sub>S\<^sub>L\<^bsup>\<ge> Suc n\<^esup>\<close> by simp
   ultimately show ?thesis
   proof -
-    have f1: \<open>(\<lbrakk> K\<^sub>1 \<not>\<Up> n \<rbrakk>\<^sub>p\<^sub>r\<^sub>i\<^sub>m \<union> \<lbrakk> K\<^sub>1 \<Up> n \<rbrakk>\<^sub>p\<^sub>r\<^sub>i\<^sub>m \<inter> \<lbrakk> K\<^sub>2 \<Up> n \<rbrakk>\<^sub>p\<^sub>r\<^sub>i\<^sub>m) \<inter> \<lbrakk> K\<^sub>1 implies K\<^sub>2 \<rbrakk>\<^sub>T\<^sub>E\<^sub>S\<^sub>L\<^bsup>\<ge> Suc n\<^esup> \<inter> (\<lbrakk>\<lbrakk> \<Psi> \<rbrakk>\<rbrakk>\<^sub>T\<^sub>E\<^sub>S\<^sub>L\<^bsup>\<ge> n\<^esup> \<inter> \<lbrakk>\<lbrakk> \<Phi> \<rbrakk>\<rbrakk>\<^sub>T\<^sub>E\<^sub>S\<^sub>L\<^bsup>\<ge> Suc n\<^esup>) = \<lbrakk>\<lbrakk> (K\<^sub>1 implies K\<^sub>2) # \<Psi> \<rbrakk>\<rbrakk>\<^sub>T\<^sub>E\<^sub>S\<^sub>L\<^bsup>\<ge> n\<^esup> \<inter> \<lbrakk>\<lbrakk> \<Phi> \<rbrakk>\<rbrakk>\<^sub>T\<^sub>E\<^sub>S\<^sub>L\<^bsup>\<ge> Suc n\<^esup>\<close>
-      using TESL_interp_stepwise_implies_coind_unfold TESL_interpretation_stepwise_cons_morph by blast
-    have \<open>\<lbrakk> K\<^sub>1 \<not>\<Up> n \<rbrakk>\<^sub>p\<^sub>r\<^sub>i\<^sub>m \<inter> \<lbrakk>\<lbrakk> \<Gamma> \<rbrakk>\<rbrakk>\<^sub>p\<^sub>r\<^sub>i\<^sub>m \<union> \<lbrakk> K\<^sub>1 \<Up> n \<rbrakk>\<^sub>p\<^sub>r\<^sub>i\<^sub>m \<inter> \<lbrakk>\<lbrakk> (K\<^sub>2 \<Up> n) # \<Gamma> \<rbrakk>\<rbrakk>\<^sub>p\<^sub>r\<^sub>i\<^sub>m = (\<lbrakk> K\<^sub>1 \<not>\<Up> n \<rbrakk>\<^sub>p\<^sub>r\<^sub>i\<^sub>m \<union> \<lbrakk> K\<^sub>1 \<Up> n \<rbrakk>\<^sub>p\<^sub>r\<^sub>i\<^sub>m \<inter> \<lbrakk> K\<^sub>2 \<Up> n \<rbrakk>\<^sub>p\<^sub>r\<^sub>i\<^sub>m) \<inter> \<lbrakk>\<lbrakk> \<Gamma> \<rbrakk>\<rbrakk>\<^sub>p\<^sub>r\<^sub>i\<^sub>m\<close>
+    have f1: \<open>(\<lbrakk> K\<^sub>1 \<not>\<Up> n \<rbrakk>\<^sub>p\<^sub>r\<^sub>i\<^sub>m \<union> \<lbrakk> K\<^sub>1 \<Up> n \<rbrakk>\<^sub>p\<^sub>r\<^sub>i\<^sub>m \<inter> \<lbrakk> K\<^sub>2 \<Up> n \<rbrakk>\<^sub>p\<^sub>r\<^sub>i\<^sub>m)
+                \<inter> \<lbrakk> K\<^sub>1 implies K\<^sub>2 \<rbrakk>\<^sub>T\<^sub>E\<^sub>S\<^sub>L\<^bsup>\<ge> Suc n\<^esup> \<inter> (\<lbrakk>\<lbrakk> \<Psi> \<rbrakk>\<rbrakk>\<^sub>T\<^sub>E\<^sub>S\<^sub>L\<^bsup>\<ge> n\<^esup>
+                \<inter> \<lbrakk>\<lbrakk> \<Phi> \<rbrakk>\<rbrakk>\<^sub>T\<^sub>E\<^sub>S\<^sub>L\<^bsup>\<ge> Suc n\<^esup>)
+              = \<lbrakk>\<lbrakk> (K\<^sub>1 implies K\<^sub>2) # \<Psi> \<rbrakk>\<rbrakk>\<^sub>T\<^sub>E\<^sub>S\<^sub>L\<^bsup>\<ge> n\<^esup> \<inter> \<lbrakk>\<lbrakk> \<Phi> \<rbrakk>\<rbrakk>\<^sub>T\<^sub>E\<^sub>S\<^sub>L\<^bsup>\<ge> Suc n\<^esup>\<close>
+      using TESL_interp_stepwise_implies_coind_unfold
+            TESL_interpretation_stepwise_cons_morph by blast
+    have \<open>\<lbrakk> K\<^sub>1 \<not>\<Up> n \<rbrakk>\<^sub>p\<^sub>r\<^sub>i\<^sub>m \<inter> \<lbrakk>\<lbrakk> \<Gamma> \<rbrakk>\<rbrakk>\<^sub>p\<^sub>r\<^sub>i\<^sub>m \<union> \<lbrakk> K\<^sub>1 \<Up> n \<rbrakk>\<^sub>p\<^sub>r\<^sub>i\<^sub>m \<inter> \<lbrakk>\<lbrakk> (K\<^sub>2 \<Up> n) # \<Gamma> \<rbrakk>\<rbrakk>\<^sub>p\<^sub>r\<^sub>i\<^sub>m
+         = (\<lbrakk> K\<^sub>1 \<not>\<Up> n \<rbrakk>\<^sub>p\<^sub>r\<^sub>i\<^sub>m \<union> \<lbrakk> K\<^sub>1 \<Up> n \<rbrakk>\<^sub>p\<^sub>r\<^sub>i\<^sub>m \<inter> \<lbrakk> K\<^sub>2 \<Up> n \<rbrakk>\<^sub>p\<^sub>r\<^sub>i\<^sub>m) \<inter> \<lbrakk>\<lbrakk> \<Gamma> \<rbrakk>\<rbrakk>\<^sub>p\<^sub>r\<^sub>i\<^sub>m\<close>
       by force
-    then have \<open>\<lbrakk> \<Gamma>, n \<turnstile> ((K\<^sub>1 implies K\<^sub>2) # \<Psi>) \<triangleright> \<Phi> \<rbrakk>\<^sub>c\<^sub>o\<^sub>n\<^sub>f\<^sub>i\<^sub>g = (\<lbrakk> K\<^sub>1 \<not>\<Up> n \<rbrakk>\<^sub>p\<^sub>r\<^sub>i\<^sub>m \<inter> \<lbrakk>\<lbrakk> \<Gamma> \<rbrakk>\<rbrakk>\<^sub>p\<^sub>r\<^sub>i\<^sub>m \<union> \<lbrakk> K\<^sub>1 \<Up> n \<rbrakk>\<^sub>p\<^sub>r\<^sub>i\<^sub>m \<inter> \<lbrakk>\<lbrakk> (K\<^sub>2 \<Up> n) # \<Gamma> \<rbrakk>\<rbrakk>\<^sub>p\<^sub>r\<^sub>i\<^sub>m) \<inter> (\<lbrakk>\<lbrakk> \<Psi> \<rbrakk>\<rbrakk>\<^sub>T\<^sub>E\<^sub>S\<^sub>L\<^bsup>\<ge> n\<^esup> \<inter> \<lbrakk>\<lbrakk> (K\<^sub>1 implies K\<^sub>2) # \<Phi> \<rbrakk>\<rbrakk>\<^sub>T\<^sub>E\<^sub>S\<^sub>L\<^bsup>\<ge> Suc n\<^esup>)\<close>
-      using f1 by (simp add: inf_left_commute inf_sup_aci(2))
-    then show ?thesis
-      by (simp add: Int_Un_distrib2 inf_sup_aci(2))
+    hence \<open>\<lbrakk> \<Gamma>, n \<turnstile> ((K\<^sub>1 implies K\<^sub>2) # \<Psi>) \<triangleright> \<Phi> \<rbrakk>\<^sub>c\<^sub>o\<^sub>n\<^sub>f\<^sub>i\<^sub>g
+      = (\<lbrakk> K\<^sub>1 \<not>\<Up> n \<rbrakk>\<^sub>p\<^sub>r\<^sub>i\<^sub>m \<inter> \<lbrakk>\<lbrakk> \<Gamma> \<rbrakk>\<rbrakk>\<^sub>p\<^sub>r\<^sub>i\<^sub>m \<union> \<lbrakk> K\<^sub>1 \<Up> n \<rbrakk>\<^sub>p\<^sub>r\<^sub>i\<^sub>m \<inter> \<lbrakk>\<lbrakk> (K\<^sub>2 \<Up> n) # \<Gamma> \<rbrakk>\<rbrakk>\<^sub>p\<^sub>r\<^sub>i\<^sub>m)
+        \<inter> (\<lbrakk>\<lbrakk> \<Psi> \<rbrakk>\<rbrakk>\<^sub>T\<^sub>E\<^sub>S\<^sub>L\<^bsup>\<ge> n\<^esup> \<inter> \<lbrakk>\<lbrakk> (K\<^sub>1 implies K\<^sub>2) # \<Phi> \<rbrakk>\<rbrakk>\<^sub>T\<^sub>E\<^sub>S\<^sub>L\<^bsup>\<ge> Suc n\<^esup>)\<close>
+      using f1 by (simp add: inf_left_commute inf_assoc)
+    thus ?thesis by (simp add: Int_Un_distrib2 inf_assoc)
   qed
 qed
 
 lemma HeronConf_interp_stepwise_implies_not_cases:
-  shows \<open>\<lbrakk> \<Gamma>, n \<turnstile> ((K\<^sub>1 implies not K\<^sub>2) # \<Psi>) \<triangleright> \<Phi> \<rbrakk>\<^sub>c\<^sub>o\<^sub>n\<^sub>f\<^sub>i\<^sub>g
-          = \<lbrakk> ((K\<^sub>1 \<not>\<Up> n) # \<Gamma>), n \<turnstile> \<Psi> \<triangleright> ((K\<^sub>1 implies not K\<^sub>2) # \<Phi>) \<rbrakk>\<^sub>c\<^sub>o\<^sub>n\<^sub>f\<^sub>i\<^sub>g
-          \<union> \<lbrakk> ((K\<^sub>1 \<Up> n) # (K\<^sub>2 \<not>\<Up> n) # \<Gamma>), n \<turnstile> \<Psi> \<triangleright> ((K\<^sub>1 implies not K\<^sub>2) # \<Phi>) \<rbrakk>\<^sub>c\<^sub>o\<^sub>n\<^sub>f\<^sub>i\<^sub>g\<close>
+   \<open>\<lbrakk> \<Gamma>, n \<turnstile> ((K\<^sub>1 implies not K\<^sub>2) # \<Psi>) \<triangleright> \<Phi> \<rbrakk>\<^sub>c\<^sub>o\<^sub>n\<^sub>f\<^sub>i\<^sub>g
+      = \<lbrakk> ((K\<^sub>1 \<not>\<Up> n) # \<Gamma>), n \<turnstile> \<Psi> \<triangleright> ((K\<^sub>1 implies not K\<^sub>2) # \<Phi>) \<rbrakk>\<^sub>c\<^sub>o\<^sub>n\<^sub>f\<^sub>i\<^sub>g
+      \<union> \<lbrakk> ((K\<^sub>1 \<Up> n) # (K\<^sub>2 \<not>\<Up> n) # \<Gamma>), n \<turnstile> \<Psi> \<triangleright> ((K\<^sub>1 implies not K\<^sub>2) # \<Phi>) \<rbrakk>\<^sub>c\<^sub>o\<^sub>n\<^sub>f\<^sub>i\<^sub>g\<close>
 proof -
-  have \<open>\<lbrakk> \<Gamma>, n \<turnstile> (K\<^sub>1 implies not K\<^sub>2) # \<Psi> \<triangleright> \<Phi> \<rbrakk>\<^sub>c\<^sub>o\<^sub>n\<^sub>f\<^sub>i\<^sub>g = \<lbrakk>\<lbrakk> \<Gamma> \<rbrakk>\<rbrakk>\<^sub>p\<^sub>r\<^sub>i\<^sub>m \<inter> \<lbrakk>\<lbrakk> (K\<^sub>1 implies not K\<^sub>2) # \<Psi> \<rbrakk>\<rbrakk>\<^sub>T\<^sub>E\<^sub>S\<^sub>L\<^bsup>\<ge> n\<^esup> \<inter> \<lbrakk>\<lbrakk> \<Phi> \<rbrakk>\<rbrakk>\<^sub>T\<^sub>E\<^sub>S\<^sub>L\<^bsup>\<ge> Suc n\<^esup>\<close>
+  have \<open>\<lbrakk> \<Gamma>, n \<turnstile> (K\<^sub>1 implies not K\<^sub>2) # \<Psi> \<triangleright> \<Phi> \<rbrakk>\<^sub>c\<^sub>o\<^sub>n\<^sub>f\<^sub>i\<^sub>g
+        = \<lbrakk>\<lbrakk> \<Gamma> \<rbrakk>\<rbrakk>\<^sub>p\<^sub>r\<^sub>i\<^sub>m \<inter> \<lbrakk>\<lbrakk> (K\<^sub>1 implies not K\<^sub>2) # \<Psi> \<rbrakk>\<rbrakk>\<^sub>T\<^sub>E\<^sub>S\<^sub>L\<^bsup>\<ge> n\<^esup> \<inter> \<lbrakk>\<lbrakk> \<Phi> \<rbrakk>\<rbrakk>\<^sub>T\<^sub>E\<^sub>S\<^sub>L\<^bsup>\<ge> Suc n\<^esup>\<close>
     by simp
   moreover have \<open>\<lbrakk> ((K\<^sub>1 \<not>\<Up> n) # \<Gamma>), n \<turnstile> \<Psi> \<triangleright> ((K\<^sub>1 implies not K\<^sub>2) # \<Phi>) \<rbrakk>\<^sub>c\<^sub>o\<^sub>n\<^sub>f\<^sub>i\<^sub>g
-                    = \<lbrakk>\<lbrakk> (K\<^sub>1 \<not>\<Up> n) # \<Gamma> \<rbrakk>\<rbrakk>\<^sub>p\<^sub>r\<^sub>i\<^sub>m \<inter> \<lbrakk>\<lbrakk> \<Psi> \<rbrakk>\<rbrakk>\<^sub>T\<^sub>E\<^sub>S\<^sub>L\<^bsup>\<ge> n\<^esup> \<inter> \<lbrakk>\<lbrakk> (K\<^sub>1 implies not K\<^sub>2) # \<Phi> \<rbrakk>\<rbrakk>\<^sub>T\<^sub>E\<^sub>S\<^sub>L\<^bsup>\<ge> Suc n\<^esup>\<close>
-    by simp
+                  = \<lbrakk>\<lbrakk> (K\<^sub>1 \<not>\<Up> n) # \<Gamma> \<rbrakk>\<rbrakk>\<^sub>p\<^sub>r\<^sub>i\<^sub>m \<inter> \<lbrakk>\<lbrakk> \<Psi> \<rbrakk>\<rbrakk>\<^sub>T\<^sub>E\<^sub>S\<^sub>L\<^bsup>\<ge> n\<^esup>
+                  \<inter> \<lbrakk>\<lbrakk> (K\<^sub>1 implies not K\<^sub>2) # \<Phi> \<rbrakk>\<rbrakk>\<^sub>T\<^sub>E\<^sub>S\<^sub>L\<^bsup>\<ge> Suc n\<^esup>\<close> by simp
   moreover have \<open>\<lbrakk> ((K\<^sub>1 \<Up> n) # (K\<^sub>2 \<not>\<Up> n) # \<Gamma>), n \<turnstile> \<Psi> \<triangleright> ((K\<^sub>1 implies not K\<^sub>2) # \<Phi>) \<rbrakk>\<^sub>c\<^sub>o\<^sub>n\<^sub>f\<^sub>i\<^sub>g
-                    = \<lbrakk>\<lbrakk> ((K\<^sub>1 \<Up> n) # (K\<^sub>2 \<not>\<Up> n) # \<Gamma>) \<rbrakk>\<rbrakk>\<^sub>p\<^sub>r\<^sub>i\<^sub>m \<inter> \<lbrakk>\<lbrakk> \<Psi> \<rbrakk>\<rbrakk>\<^sub>T\<^sub>E\<^sub>S\<^sub>L\<^bsup>\<ge> n\<^esup> \<inter> \<lbrakk>\<lbrakk> (K\<^sub>1 implies not K\<^sub>2) # \<Phi> \<rbrakk>\<rbrakk>\<^sub>T\<^sub>E\<^sub>S\<^sub>L\<^bsup>\<ge> Suc n\<^esup>\<close>
-    by simp
+                  = \<lbrakk>\<lbrakk> ((K\<^sub>1 \<Up> n) # (K\<^sub>2 \<not>\<Up> n) # \<Gamma>) \<rbrakk>\<rbrakk>\<^sub>p\<^sub>r\<^sub>i\<^sub>m \<inter> \<lbrakk>\<lbrakk> \<Psi> \<rbrakk>\<rbrakk>\<^sub>T\<^sub>E\<^sub>S\<^sub>L\<^bsup>\<ge> n\<^esup>
+                  \<inter> \<lbrakk>\<lbrakk> (K\<^sub>1 implies not K\<^sub>2) # \<Phi> \<rbrakk>\<rbrakk>\<^sub>T\<^sub>E\<^sub>S\<^sub>L\<^bsup>\<ge> Suc n\<^esup>\<close> by simp
   ultimately show ?thesis
   proof -
-    have f1: \<open>(\<lbrakk> K\<^sub>1 \<not>\<Up> n \<rbrakk>\<^sub>p\<^sub>r\<^sub>i\<^sub>m \<union> \<lbrakk> K\<^sub>1 \<Up> n \<rbrakk>\<^sub>p\<^sub>r\<^sub>i\<^sub>m \<inter> \<lbrakk> K\<^sub>2 \<not>\<Up> n \<rbrakk>\<^sub>p\<^sub>r\<^sub>i\<^sub>m) \<inter> \<lbrakk> K\<^sub>1 implies not K\<^sub>2 \<rbrakk>\<^sub>T\<^sub>E\<^sub>S\<^sub>L\<^bsup>\<ge> Suc n\<^esup> \<inter> (\<lbrakk>\<lbrakk> \<Psi> \<rbrakk>\<rbrakk>\<^sub>T\<^sub>E\<^sub>S\<^sub>L\<^bsup>\<ge> n\<^esup> \<inter> \<lbrakk>\<lbrakk> \<Phi> \<rbrakk>\<rbrakk>\<^sub>T\<^sub>E\<^sub>S\<^sub>L\<^bsup>\<ge> Suc n\<^esup>)
-                = \<lbrakk>\<lbrakk> (K\<^sub>1 implies not K\<^sub>2) # \<Psi> \<rbrakk>\<rbrakk>\<^sub>T\<^sub>E\<^sub>S\<^sub>L\<^bsup>\<ge> n\<^esup> \<inter> \<lbrakk>\<lbrakk> \<Phi> \<rbrakk>\<rbrakk>\<^sub>T\<^sub>E\<^sub>S\<^sub>L\<^bsup>\<ge> Suc n\<^esup>\<close>
-      using TESL_interp_stepwise_implies_not_coind_unfold TESL_interpretation_stepwise_cons_morph by blast
-    have \<open>\<lbrakk> K\<^sub>1 \<not>\<Up> n \<rbrakk>\<^sub>p\<^sub>r\<^sub>i\<^sub>m \<inter> \<lbrakk>\<lbrakk> \<Gamma> \<rbrakk>\<rbrakk>\<^sub>p\<^sub>r\<^sub>i\<^sub>m \<union> \<lbrakk> K\<^sub>1 \<Up> n \<rbrakk>\<^sub>p\<^sub>r\<^sub>i\<^sub>m \<inter> \<lbrakk>\<lbrakk> (K\<^sub>2 \<not>\<Up> n) # \<Gamma> \<rbrakk>\<rbrakk>\<^sub>p\<^sub>r\<^sub>i\<^sub>m = (\<lbrakk> K\<^sub>1 \<not>\<Up> n \<rbrakk>\<^sub>p\<^sub>r\<^sub>i\<^sub>m \<union> \<lbrakk> K\<^sub>1 \<Up> n \<rbrakk>\<^sub>p\<^sub>r\<^sub>i\<^sub>m \<inter> \<lbrakk> K\<^sub>2 \<not>\<Up> n \<rbrakk>\<^sub>p\<^sub>r\<^sub>i\<^sub>m) \<inter> \<lbrakk>\<lbrakk> \<Gamma> \<rbrakk>\<rbrakk>\<^sub>p\<^sub>r\<^sub>i\<^sub>m\<close>
+    have f1: \<open>(\<lbrakk> K\<^sub>1 \<not>\<Up> n \<rbrakk>\<^sub>p\<^sub>r\<^sub>i\<^sub>m \<union> \<lbrakk> K\<^sub>1 \<Up> n \<rbrakk>\<^sub>p\<^sub>r\<^sub>i\<^sub>m \<inter> \<lbrakk> K\<^sub>2 \<not>\<Up> n \<rbrakk>\<^sub>p\<^sub>r\<^sub>i\<^sub>m)
+              \<inter> \<lbrakk> K\<^sub>1 implies not K\<^sub>2 \<rbrakk>\<^sub>T\<^sub>E\<^sub>S\<^sub>L\<^bsup>\<ge> Suc n\<^esup>
+              \<inter> (\<lbrakk>\<lbrakk> \<Psi> \<rbrakk>\<rbrakk>\<^sub>T\<^sub>E\<^sub>S\<^sub>L\<^bsup>\<ge> n\<^esup> \<inter> \<lbrakk>\<lbrakk> \<Phi> \<rbrakk>\<rbrakk>\<^sub>T\<^sub>E\<^sub>S\<^sub>L\<^bsup>\<ge> Suc n\<^esup>)
+              = \<lbrakk>\<lbrakk> (K\<^sub>1 implies not K\<^sub>2) # \<Psi> \<rbrakk>\<rbrakk>\<^sub>T\<^sub>E\<^sub>S\<^sub>L\<^bsup>\<ge> n\<^esup> \<inter> \<lbrakk>\<lbrakk> \<Phi> \<rbrakk>\<rbrakk>\<^sub>T\<^sub>E\<^sub>S\<^sub>L\<^bsup>\<ge> Suc n\<^esup>\<close>
+      using TESL_interp_stepwise_implies_not_coind_unfold
+            TESL_interpretation_stepwise_cons_morph by blast
+    have \<open>\<lbrakk> K\<^sub>1 \<not>\<Up> n \<rbrakk>\<^sub>p\<^sub>r\<^sub>i\<^sub>m \<inter> \<lbrakk>\<lbrakk> \<Gamma> \<rbrakk>\<rbrakk>\<^sub>p\<^sub>r\<^sub>i\<^sub>m \<union> \<lbrakk> K\<^sub>1 \<Up> n \<rbrakk>\<^sub>p\<^sub>r\<^sub>i\<^sub>m \<inter> \<lbrakk>\<lbrakk> (K\<^sub>2 \<not>\<Up> n) # \<Gamma> \<rbrakk>\<rbrakk>\<^sub>p\<^sub>r\<^sub>i\<^sub>m
+           = (\<lbrakk> K\<^sub>1 \<not>\<Up> n \<rbrakk>\<^sub>p\<^sub>r\<^sub>i\<^sub>m \<union> \<lbrakk> K\<^sub>1 \<Up> n \<rbrakk>\<^sub>p\<^sub>r\<^sub>i\<^sub>m \<inter> \<lbrakk> K\<^sub>2 \<not>\<Up> n \<rbrakk>\<^sub>p\<^sub>r\<^sub>i\<^sub>m) \<inter> \<lbrakk>\<lbrakk> \<Gamma> \<rbrakk>\<rbrakk>\<^sub>p\<^sub>r\<^sub>i\<^sub>m\<close>
       by force
     then have \<open>\<lbrakk> \<Gamma>, n \<turnstile> ((K\<^sub>1 implies not K\<^sub>2) # \<Psi>) \<triangleright> \<Phi> \<rbrakk>\<^sub>c\<^sub>o\<^sub>n\<^sub>f\<^sub>i\<^sub>g
-                 = (\<lbrakk> K\<^sub>1 \<not>\<Up> n \<rbrakk>\<^sub>p\<^sub>r\<^sub>i\<^sub>m \<inter> \<lbrakk>\<lbrakk> \<Gamma> \<rbrakk>\<rbrakk>\<^sub>p\<^sub>r\<^sub>i\<^sub>m \<union> \<lbrakk> K\<^sub>1 \<Up> n \<rbrakk>\<^sub>p\<^sub>r\<^sub>i\<^sub>m \<inter> \<lbrakk>\<lbrakk> (K\<^sub>2 \<not>\<Up> n) # \<Gamma> \<rbrakk>\<rbrakk>\<^sub>p\<^sub>r\<^sub>i\<^sub>m) \<inter> (\<lbrakk>\<lbrakk> \<Psi> \<rbrakk>\<rbrakk>\<^sub>T\<^sub>E\<^sub>S\<^sub>L\<^bsup>\<ge> n\<^esup> \<inter> \<lbrakk>\<lbrakk> (K\<^sub>1 implies not K\<^sub>2) # \<Phi> \<rbrakk>\<rbrakk>\<^sub>T\<^sub>E\<^sub>S\<^sub>L\<^bsup>\<ge> Suc n\<^esup>)\<close>
-      using f1 by (simp add: inf_left_commute inf_sup_aci(2))
-    then show ?thesis
-      by (simp add: Int_Un_distrib2 inf_sup_aci(2))
+                 = (\<lbrakk> K\<^sub>1 \<not>\<Up> n \<rbrakk>\<^sub>p\<^sub>r\<^sub>i\<^sub>m \<inter> \<lbrakk>\<lbrakk> \<Gamma> \<rbrakk>\<rbrakk>\<^sub>p\<^sub>r\<^sub>i\<^sub>m \<union> \<lbrakk> K\<^sub>1 \<Up> n \<rbrakk>\<^sub>p\<^sub>r\<^sub>i\<^sub>m
+                    \<inter> \<lbrakk>\<lbrakk> (K\<^sub>2 \<not>\<Up> n) # \<Gamma> \<rbrakk>\<rbrakk>\<^sub>p\<^sub>r\<^sub>i\<^sub>m) \<inter> (\<lbrakk>\<lbrakk> \<Psi> \<rbrakk>\<rbrakk>\<^sub>T\<^sub>E\<^sub>S\<^sub>L\<^bsup>\<ge> n\<^esup>
+                    \<inter> \<lbrakk>\<lbrakk> (K\<^sub>1 implies not K\<^sub>2) # \<Phi> \<rbrakk>\<rbrakk>\<^sub>T\<^sub>E\<^sub>S\<^sub>L\<^bsup>\<ge> Suc n\<^esup>)\<close>
+      using f1 by (simp add: inf_left_commute inf_assoc)
+    thus ?thesis by (simp add: Int_Un_distrib2 inf_assoc)
   qed
 qed
 
 lemma HeronConf_interp_stepwise_timedelayed_cases:
-  shows \<open>\<lbrakk> \<Gamma>, n \<turnstile> ((K\<^sub>1 time-delayed by \<delta>\<tau> on K\<^sub>2 implies K\<^sub>3) # \<Psi>) \<triangleright> \<Phi> \<rbrakk>\<^sub>c\<^sub>o\<^sub>n\<^sub>f\<^sub>i\<^sub>g
-          = \<lbrakk> ((K\<^sub>1 \<not>\<Up> n) # \<Gamma>), n \<turnstile> \<Psi> \<triangleright> ((K\<^sub>1 time-delayed by \<delta>\<tau> on K\<^sub>2 implies K\<^sub>3) # \<Phi>) \<rbrakk>\<^sub>c\<^sub>o\<^sub>n\<^sub>f\<^sub>i\<^sub>g
-          \<union> \<lbrakk> ((K\<^sub>1 \<Up> n) # (K\<^sub>2 @ n \<oplus> \<delta>\<tau> \<Rightarrow> K\<^sub>3) # \<Gamma>), n \<turnstile> \<Psi> \<triangleright> ((K\<^sub>1 time-delayed by \<delta>\<tau> on K\<^sub>2 implies K\<^sub>3) # \<Phi>) \<rbrakk>\<^sub>c\<^sub>o\<^sub>n\<^sub>f\<^sub>i\<^sub>g\<close>
+  \<open>\<lbrakk> \<Gamma>, n \<turnstile> ((K\<^sub>1 time-delayed by \<delta>\<tau> on K\<^sub>2 implies K\<^sub>3) # \<Psi>) \<triangleright> \<Phi> \<rbrakk>\<^sub>c\<^sub>o\<^sub>n\<^sub>f\<^sub>i\<^sub>g
+    = \<lbrakk> ((K\<^sub>1 \<not>\<Up> n) # \<Gamma>), n \<turnstile> \<Psi> \<triangleright> ((K\<^sub>1 time-delayed by \<delta>\<tau> on K\<^sub>2 implies K\<^sub>3) # \<Phi>) \<rbrakk>\<^sub>c\<^sub>o\<^sub>n\<^sub>f\<^sub>i\<^sub>g
+    \<union> \<lbrakk> ((K\<^sub>1 \<Up> n) # (K\<^sub>2 @ n \<oplus> \<delta>\<tau> \<Rightarrow> K\<^sub>3) # \<Gamma>), n
+        \<turnstile> \<Psi> \<triangleright> ((K\<^sub>1 time-delayed by \<delta>\<tau> on K\<^sub>2 implies K\<^sub>3) # \<Phi>) \<rbrakk>\<^sub>c\<^sub>o\<^sub>n\<^sub>f\<^sub>i\<^sub>g\<close>
 proof -
   have 1:\<open>\<lbrakk> \<Gamma>, n \<turnstile> (K\<^sub>1 time-delayed by \<delta>\<tau> on K\<^sub>2 implies K\<^sub>3) # \<Psi> \<triangleright> \<Phi> \<rbrakk>\<^sub>c\<^sub>o\<^sub>n\<^sub>f\<^sub>i\<^sub>g
-         = \<lbrakk>\<lbrakk> \<Gamma> \<rbrakk>\<rbrakk>\<^sub>p\<^sub>r\<^sub>i\<^sub>m \<inter> \<lbrakk>\<lbrakk> (K\<^sub>1 time-delayed by \<delta>\<tau> on K\<^sub>2 implies K\<^sub>3) # \<Psi> \<rbrakk>\<rbrakk>\<^sub>T\<^sub>E\<^sub>S\<^sub>L\<^bsup>\<ge> n\<^esup> \<inter> \<lbrakk>\<lbrakk> \<Phi> \<rbrakk>\<rbrakk>\<^sub>T\<^sub>E\<^sub>S\<^sub>L\<^bsup>\<ge> Suc n\<^esup>\<close>
+         = \<lbrakk>\<lbrakk> \<Gamma> \<rbrakk>\<rbrakk>\<^sub>p\<^sub>r\<^sub>i\<^sub>m \<inter> \<lbrakk>\<lbrakk> (K\<^sub>1 time-delayed by \<delta>\<tau> on K\<^sub>2 implies K\<^sub>3) # \<Psi> \<rbrakk>\<rbrakk>\<^sub>T\<^sub>E\<^sub>S\<^sub>L\<^bsup>\<ge> n\<^esup>
+          \<inter> \<lbrakk>\<lbrakk> \<Phi> \<rbrakk>\<rbrakk>\<^sub>T\<^sub>E\<^sub>S\<^sub>L\<^bsup>\<ge> Suc n\<^esup>\<close> by simp
+  moreover have \<open>\<lbrakk> ((K\<^sub>1 \<not>\<Up> n) # \<Gamma>), n
+                  \<turnstile> \<Psi> \<triangleright> ((K\<^sub>1 time-delayed by \<delta>\<tau> on K\<^sub>2 implies K\<^sub>3) # \<Phi>) \<rbrakk>\<^sub>c\<^sub>o\<^sub>n\<^sub>f\<^sub>i\<^sub>g
+                 = \<lbrakk>\<lbrakk> (K\<^sub>1 \<not>\<Up> n) # \<Gamma> \<rbrakk>\<rbrakk>\<^sub>p\<^sub>r\<^sub>i\<^sub>m \<inter> \<lbrakk>\<lbrakk> \<Psi> \<rbrakk>\<rbrakk>\<^sub>T\<^sub>E\<^sub>S\<^sub>L\<^bsup>\<ge> n\<^esup>
+                  \<inter> \<lbrakk>\<lbrakk> (K\<^sub>1 time-delayed by \<delta>\<tau> on K\<^sub>2 implies K\<^sub>3) # \<Phi> \<rbrakk>\<rbrakk>\<^sub>T\<^sub>E\<^sub>S\<^sub>L\<^bsup>\<ge> Suc n\<^esup>\<close>
     by simp
-  moreover have \<open>\<lbrakk> ((K\<^sub>1 \<not>\<Up> n) # \<Gamma>), n \<turnstile> \<Psi> \<triangleright> ((K\<^sub>1 time-delayed by \<delta>\<tau> on K\<^sub>2 implies K\<^sub>3) # \<Phi>) \<rbrakk>\<^sub>c\<^sub>o\<^sub>n\<^sub>f\<^sub>i\<^sub>g
-                   = \<lbrakk>\<lbrakk> (K\<^sub>1 \<not>\<Up> n) # \<Gamma> \<rbrakk>\<rbrakk>\<^sub>p\<^sub>r\<^sub>i\<^sub>m \<inter> \<lbrakk>\<lbrakk> \<Psi> \<rbrakk>\<rbrakk>\<^sub>T\<^sub>E\<^sub>S\<^sub>L\<^bsup>\<ge> n\<^esup> \<inter> \<lbrakk>\<lbrakk> (K\<^sub>1 time-delayed by \<delta>\<tau> on K\<^sub>2 implies K\<^sub>3) # \<Phi> \<rbrakk>\<rbrakk>\<^sub>T\<^sub>E\<^sub>S\<^sub>L\<^bsup>\<ge> Suc n\<^esup>\<close>
-    by simp
-  moreover have \<open>\<lbrakk> ((K\<^sub>1 \<Up> n) # (K\<^sub>2 @ n \<oplus> \<delta>\<tau> \<Rightarrow> K\<^sub>3) # \<Gamma>), n \<turnstile> \<Psi> \<triangleright> ((K\<^sub>1 time-delayed by \<delta>\<tau> on K\<^sub>2 implies K\<^sub>3) # \<Phi>) \<rbrakk>\<^sub>c\<^sub>o\<^sub>n\<^sub>f\<^sub>i\<^sub>g
-                   = \<lbrakk>\<lbrakk> (K\<^sub>1 \<Up> n) # (K\<^sub>2 @ n \<oplus> \<delta>\<tau> \<Rightarrow> K\<^sub>3) # \<Gamma> \<rbrakk>\<rbrakk>\<^sub>p\<^sub>r\<^sub>i\<^sub>m \<inter> \<lbrakk>\<lbrakk> \<Psi> \<rbrakk>\<rbrakk>\<^sub>T\<^sub>E\<^sub>S\<^sub>L\<^bsup>\<ge> n\<^esup>
-                   \<inter> \<lbrakk>\<lbrakk> (K\<^sub>1 time-delayed by \<delta>\<tau> on K\<^sub>2 implies K\<^sub>3) # \<Phi> \<rbrakk>\<rbrakk>\<^sub>T\<^sub>E\<^sub>S\<^sub>L\<^bsup>\<ge> Suc n\<^esup>\<close>
+  moreover have \<open>\<lbrakk> ((K\<^sub>1 \<Up> n) # (K\<^sub>2 @ n \<oplus> \<delta>\<tau> \<Rightarrow> K\<^sub>3) # \<Gamma>), n
+                  \<turnstile> \<Psi> \<triangleright> ((K\<^sub>1 time-delayed by \<delta>\<tau> on K\<^sub>2 implies K\<^sub>3) # \<Phi>) \<rbrakk>\<^sub>c\<^sub>o\<^sub>n\<^sub>f\<^sub>i\<^sub>g
+                 = \<lbrakk>\<lbrakk> (K\<^sub>1 \<Up> n) # (K\<^sub>2 @ n \<oplus> \<delta>\<tau> \<Rightarrow> K\<^sub>3) # \<Gamma> \<rbrakk>\<rbrakk>\<^sub>p\<^sub>r\<^sub>i\<^sub>m \<inter> \<lbrakk>\<lbrakk> \<Psi> \<rbrakk>\<rbrakk>\<^sub>T\<^sub>E\<^sub>S\<^sub>L\<^bsup>\<ge> n\<^esup>
+                  \<inter> \<lbrakk>\<lbrakk> (K\<^sub>1 time-delayed by \<delta>\<tau> on K\<^sub>2 implies K\<^sub>3) # \<Phi> \<rbrakk>\<rbrakk>\<^sub>T\<^sub>E\<^sub>S\<^sub>L\<^bsup>\<ge> Suc n\<^esup>\<close>
     by simp
   ultimately show ?thesis
   proof -
-    have \<open>\<lbrakk> \<Gamma>, n \<turnstile> (K\<^sub>1 time-delayed by \<delta>\<tau> on K\<^sub>2 implies K\<^sub>3) # \<Psi> \<triangleright> \<Phi> \<rbrakk>\<^sub>c\<^sub>o\<^sub>n\<^sub>f\<^sub>i\<^sub>g = \<lbrakk>\<lbrakk> \<Gamma> \<rbrakk>\<rbrakk>\<^sub>p\<^sub>r\<^sub>i\<^sub>m \<inter> (\<lbrakk>\<lbrakk> (K\<^sub>1 time-delayed by \<delta>\<tau> on K\<^sub>2 implies K\<^sub>3) # \<Psi> \<rbrakk>\<rbrakk>\<^sub>T\<^sub>E\<^sub>S\<^sub>L\<^bsup>\<ge> n\<^esup> \<inter> \<lbrakk>\<lbrakk> \<Phi> \<rbrakk>\<rbrakk>\<^sub>T\<^sub>E\<^sub>S\<^sub>L\<^bsup>\<ge> Suc n\<^esup>)\<close>
+    have \<open>\<lbrakk> \<Gamma>, n \<turnstile> (K\<^sub>1 time-delayed by \<delta>\<tau> on K\<^sub>2 implies K\<^sub>3) # \<Psi> \<triangleright> \<Phi> \<rbrakk>\<^sub>c\<^sub>o\<^sub>n\<^sub>f\<^sub>i\<^sub>g
+      = \<lbrakk>\<lbrakk> \<Gamma> \<rbrakk>\<rbrakk>\<^sub>p\<^sub>r\<^sub>i\<^sub>m \<inter> (\<lbrakk>\<lbrakk> (K\<^sub>1 time-delayed by \<delta>\<tau> on K\<^sub>2 implies K\<^sub>3) # \<Psi> \<rbrakk>\<rbrakk>\<^sub>T\<^sub>E\<^sub>S\<^sub>L\<^bsup>\<ge> n\<^esup>
+        \<inter> \<lbrakk>\<lbrakk> \<Phi> \<rbrakk>\<rbrakk>\<^sub>T\<^sub>E\<^sub>S\<^sub>L\<^bsup>\<ge> Suc n\<^esup>)\<close>
       using 1 by blast
-    then have \<open>\<lbrakk> \<Gamma>, n \<turnstile> (K\<^sub>1 time-delayed by \<delta>\<tau> on K\<^sub>2 implies K\<^sub>3) # \<Psi> \<triangleright> \<Phi> \<rbrakk>\<^sub>c\<^sub>o\<^sub>n\<^sub>f\<^sub>i\<^sub>g = (\<lbrakk> K\<^sub>1 \<not>\<Up> n \<rbrakk>\<^sub>p\<^sub>r\<^sub>i\<^sub>m \<union> \<lbrakk> K\<^sub>1 \<Up> n \<rbrakk>\<^sub>p\<^sub>r\<^sub>i\<^sub>m \<inter> \<lbrakk> K\<^sub>2 @ n \<oplus> \<delta>\<tau> \<Rightarrow> K\<^sub>3 \<rbrakk>\<^sub>p\<^sub>r\<^sub>i\<^sub>m) \<inter> (\<lbrakk>\<lbrakk> \<Gamma> \<rbrakk>\<rbrakk>\<^sub>p\<^sub>r\<^sub>i\<^sub>m \<inter> (\<lbrakk>\<lbrakk> \<Psi> \<rbrakk>\<rbrakk>\<^sub>T\<^sub>E\<^sub>S\<^sub>L\<^bsup>\<ge> n\<^esup> \<inter> \<lbrakk>\<lbrakk> (K\<^sub>1 time-delayed by \<delta>\<tau> on K\<^sub>2 implies K\<^sub>3) # \<Phi> \<rbrakk>\<rbrakk>\<^sub>T\<^sub>E\<^sub>S\<^sub>L\<^bsup>\<ge> Suc n\<^esup>))\<close>
-      using TESL_interpretation_stepwise_cons_morph TESL_interp_stepwise_timedelayed_coind_unfold
+    hence \<open>\<lbrakk> \<Gamma>, n \<turnstile> (K\<^sub>1 time-delayed by \<delta>\<tau> on K\<^sub>2 implies K\<^sub>3) # \<Psi> \<triangleright> \<Phi> \<rbrakk>\<^sub>c\<^sub>o\<^sub>n\<^sub>f\<^sub>i\<^sub>g
+          = (\<lbrakk> K\<^sub>1 \<not>\<Up> n \<rbrakk>\<^sub>p\<^sub>r\<^sub>i\<^sub>m \<union> \<lbrakk> K\<^sub>1 \<Up> n \<rbrakk>\<^sub>p\<^sub>r\<^sub>i\<^sub>m \<inter> \<lbrakk> K\<^sub>2 @ n \<oplus> \<delta>\<tau> \<Rightarrow> K\<^sub>3 \<rbrakk>\<^sub>p\<^sub>r\<^sub>i\<^sub>m)
+            \<inter> (\<lbrakk>\<lbrakk> \<Gamma> \<rbrakk>\<rbrakk>\<^sub>p\<^sub>r\<^sub>i\<^sub>m \<inter> (\<lbrakk>\<lbrakk> \<Psi> \<rbrakk>\<rbrakk>\<^sub>T\<^sub>E\<^sub>S\<^sub>L\<^bsup>\<ge> n\<^esup>
+            \<inter> \<lbrakk>\<lbrakk> (K\<^sub>1 time-delayed by \<delta>\<tau> on K\<^sub>2 implies K\<^sub>3) # \<Phi> \<rbrakk>\<rbrakk>\<^sub>T\<^sub>E\<^sub>S\<^sub>L\<^bsup>\<ge> Suc n\<^esup>))\<close>
+      using TESL_interpretation_stepwise_cons_morph
+            TESL_interp_stepwise_timedelayed_coind_unfold
     proof -
-      have \<open>\<lbrakk>\<lbrakk> (K\<^sub>1 time-delayed by \<delta>\<tau> on K\<^sub>2 implies K\<^sub>3) # \<Psi> \<rbrakk>\<rbrakk>\<^sub>T\<^sub>E\<^sub>S\<^sub>L\<^bsup>\<ge> n\<^esup> = (\<lbrakk> K\<^sub>1 \<not>\<Up> n \<rbrakk>\<^sub>p\<^sub>r\<^sub>i\<^sub>m \<union> \<lbrakk> K\<^sub>1 \<Up> n \<rbrakk>\<^sub>p\<^sub>r\<^sub>i\<^sub>m \<inter> \<lbrakk> K\<^sub>2 @ n \<oplus> \<delta>\<tau> \<Rightarrow> K\<^sub>3 \<rbrakk>\<^sub>p\<^sub>r\<^sub>i\<^sub>m) \<inter> \<lbrakk> K\<^sub>1 time-delayed by \<delta>\<tau> on K\<^sub>2 implies K\<^sub>3 \<rbrakk>\<^sub>T\<^sub>E\<^sub>S\<^sub>L\<^bsup>\<ge> Suc n\<^esup> \<inter> \<lbrakk>\<lbrakk> \<Psi> \<rbrakk>\<rbrakk>\<^sub>T\<^sub>E\<^sub>S\<^sub>L\<^bsup>\<ge> n\<^esup>\<close>
-        using TESL_interp_stepwise_timedelayed_coind_unfold TESL_interpretation_stepwise_cons_morph by blast
+      have \<open>\<lbrakk>\<lbrakk> (K\<^sub>1 time-delayed by \<delta>\<tau> on K\<^sub>2 implies K\<^sub>3) # \<Psi> \<rbrakk>\<rbrakk>\<^sub>T\<^sub>E\<^sub>S\<^sub>L\<^bsup>\<ge> n\<^esup>
+            = (\<lbrakk> K\<^sub>1 \<not>\<Up> n \<rbrakk>\<^sub>p\<^sub>r\<^sub>i\<^sub>m \<union> \<lbrakk> K\<^sub>1 \<Up> n \<rbrakk>\<^sub>p\<^sub>r\<^sub>i\<^sub>m \<inter> \<lbrakk> K\<^sub>2 @ n \<oplus> \<delta>\<tau> \<Rightarrow> K\<^sub>3 \<rbrakk>\<^sub>p\<^sub>r\<^sub>i\<^sub>m)
+            \<inter> \<lbrakk> K\<^sub>1 time-delayed by \<delta>\<tau> on K\<^sub>2 implies K\<^sub>3 \<rbrakk>\<^sub>T\<^sub>E\<^sub>S\<^sub>L\<^bsup>\<ge> Suc n\<^esup> \<inter> \<lbrakk>\<lbrakk> \<Psi> \<rbrakk>\<rbrakk>\<^sub>T\<^sub>E\<^sub>S\<^sub>L\<^bsup>\<ge> n\<^esup>\<close>
+        using TESL_interp_stepwise_timedelayed_coind_unfold
+              TESL_interpretation_stepwise_cons_morph by blast
       then show ?thesis
         by (simp add: Int_assoc Int_left_commute)
     qed
@@ -469,63 +531,75 @@ proof -
 qed
 
 lemma HeronConf_interp_stepwise_weakly_precedes_cases:
-  shows \<open>\<lbrakk> \<Gamma>, n \<turnstile> ((K\<^sub>1 weakly precedes K\<^sub>2) # \<Psi>) \<triangleright> \<Phi> \<rbrakk>\<^sub>c\<^sub>o\<^sub>n\<^sub>f\<^sub>i\<^sub>g
-          = \<lbrakk> ((\<lceil>#\<^sup>\<le> K\<^sub>2 n, #\<^sup>\<le> K\<^sub>1 n\<rceil> \<in> (\<lambda>(x,y). x\<le>y)) # \<Gamma>), n \<turnstile> \<Psi> \<triangleright> ((K\<^sub>1 weakly precedes K\<^sub>2) # \<Phi>) \<rbrakk>\<^sub>c\<^sub>o\<^sub>n\<^sub>f\<^sub>i\<^sub>g\<close>
+   \<open>\<lbrakk> \<Gamma>, n \<turnstile> ((K\<^sub>1 weakly precedes K\<^sub>2) # \<Psi>) \<triangleright> \<Phi> \<rbrakk>\<^sub>c\<^sub>o\<^sub>n\<^sub>f\<^sub>i\<^sub>g
+    = \<lbrakk> ((\<lceil>#\<^sup>\<le> K\<^sub>2 n, #\<^sup>\<le> K\<^sub>1 n\<rceil> \<in> (\<lambda>(x,y). x\<le>y)) # \<Gamma>), n
+      \<turnstile> \<Psi> \<triangleright> ((K\<^sub>1 weakly precedes K\<^sub>2) # \<Phi>) \<rbrakk>\<^sub>c\<^sub>o\<^sub>n\<^sub>f\<^sub>i\<^sub>g\<close>
 proof -
-  have \<open>\<lbrakk> \<Gamma>, n \<turnstile> (K\<^sub>1 weakly precedes K\<^sub>2) # \<Psi> \<triangleright> \<Phi> \<rbrakk>\<^sub>c\<^sub>o\<^sub>n\<^sub>f\<^sub>i\<^sub>g = \<lbrakk>\<lbrakk> \<Gamma> \<rbrakk>\<rbrakk>\<^sub>p\<^sub>r\<^sub>i\<^sub>m \<inter> \<lbrakk>\<lbrakk> (K\<^sub>1 weakly precedes K\<^sub>2) # \<Psi> \<rbrakk>\<rbrakk>\<^sub>T\<^sub>E\<^sub>S\<^sub>L\<^bsup>\<ge> n\<^esup> \<inter> \<lbrakk>\<lbrakk> \<Phi> \<rbrakk>\<rbrakk>\<^sub>T\<^sub>E\<^sub>S\<^sub>L\<^bsup>\<ge> Suc n\<^esup>\<close>
-    by simp
-  moreover have \<open>\<lbrakk> ((\<lceil>#\<^sup>\<le> K\<^sub>2 n, #\<^sup>\<le> K\<^sub>1 n\<rceil> \<in> (\<lambda>(x,y). x\<le>y)) # \<Gamma>), n \<turnstile> \<Psi> \<triangleright> ((K\<^sub>1 weakly precedes K\<^sub>2) # \<Phi>) \<rbrakk>\<^sub>c\<^sub>o\<^sub>n\<^sub>f\<^sub>i\<^sub>g
-                    = \<lbrakk>\<lbrakk> (\<lceil>#\<^sup>\<le> K\<^sub>2 n, #\<^sup>\<le> K\<^sub>1 n\<rceil> \<in> (\<lambda>(x,y). x\<le>y)) # \<Gamma> \<rbrakk>\<rbrakk>\<^sub>p\<^sub>r\<^sub>i\<^sub>m \<inter> \<lbrakk>\<lbrakk> \<Psi> \<rbrakk>\<rbrakk>\<^sub>T\<^sub>E\<^sub>S\<^sub>L\<^bsup>\<ge> n\<^esup> \<inter> \<lbrakk>\<lbrakk> (K\<^sub>1 weakly precedes K\<^sub>2) # \<Phi> \<rbrakk>\<rbrakk>\<^sub>T\<^sub>E\<^sub>S\<^sub>L\<^bsup>\<ge> Suc n\<^esup>\<close>
+  have \<open>\<lbrakk> \<Gamma>, n \<turnstile> (K\<^sub>1 weakly precedes K\<^sub>2) # \<Psi> \<triangleright> \<Phi> \<rbrakk>\<^sub>c\<^sub>o\<^sub>n\<^sub>f\<^sub>i\<^sub>g
+        = \<lbrakk>\<lbrakk> \<Gamma> \<rbrakk>\<rbrakk>\<^sub>p\<^sub>r\<^sub>i\<^sub>m \<inter> \<lbrakk>\<lbrakk> (K\<^sub>1 weakly precedes K\<^sub>2) # \<Psi> \<rbrakk>\<rbrakk>\<^sub>T\<^sub>E\<^sub>S\<^sub>L\<^bsup>\<ge> n\<^esup>
+          \<inter> \<lbrakk>\<lbrakk> \<Phi> \<rbrakk>\<rbrakk>\<^sub>T\<^sub>E\<^sub>S\<^sub>L\<^bsup>\<ge> Suc n\<^esup>\<close> by simp
+  moreover have \<open>\<lbrakk> ((\<lceil>#\<^sup>\<le> K\<^sub>2 n, #\<^sup>\<le> K\<^sub>1 n\<rceil> \<in> (\<lambda>(x,y). x\<le>y)) # \<Gamma>), n
+                  \<turnstile> \<Psi> \<triangleright> ((K\<^sub>1 weakly precedes K\<^sub>2) # \<Phi>) \<rbrakk>\<^sub>c\<^sub>o\<^sub>n\<^sub>f\<^sub>i\<^sub>g
+                = \<lbrakk>\<lbrakk> (\<lceil>#\<^sup>\<le> K\<^sub>2 n, #\<^sup>\<le> K\<^sub>1 n\<rceil> \<in> (\<lambda>(x,y). x\<le>y)) # \<Gamma> \<rbrakk>\<rbrakk>\<^sub>p\<^sub>r\<^sub>i\<^sub>m
+                \<inter> \<lbrakk>\<lbrakk> \<Psi> \<rbrakk>\<rbrakk>\<^sub>T\<^sub>E\<^sub>S\<^sub>L\<^bsup>\<ge> n\<^esup> \<inter> \<lbrakk>\<lbrakk> (K\<^sub>1 weakly precedes K\<^sub>2) # \<Phi> \<rbrakk>\<rbrakk>\<^sub>T\<^sub>E\<^sub>S\<^sub>L\<^bsup>\<ge> Suc n\<^esup>\<close>
     by simp
   ultimately show ?thesis
   proof -
-    have \<open>\<lbrakk> \<lceil>#\<^sup>\<le> K\<^sub>2 n, #\<^sup>\<le> K\<^sub>1 n\<rceil> \<in> (\<lambda>(x,y). x\<le>y) \<rbrakk>\<^sub>p\<^sub>r\<^sub>i\<^sub>m \<inter> \<lbrakk> K\<^sub>1 weakly precedes K\<^sub>2 \<rbrakk>\<^sub>T\<^sub>E\<^sub>S\<^sub>L\<^bsup>\<ge> Suc n\<^esup> \<inter> \<lbrakk>\<lbrakk> \<Psi> \<rbrakk>\<rbrakk>\<^sub>T\<^sub>E\<^sub>S\<^sub>L\<^bsup>\<ge> n\<^esup> = \<lbrakk>\<lbrakk> (K\<^sub>1 weakly precedes K\<^sub>2) # \<Psi> \<rbrakk>\<rbrakk>\<^sub>T\<^sub>E\<^sub>S\<^sub>L\<^bsup>\<ge> n\<^esup>\<close>
-      using TESL_interp_stepwise_weakly_precedes_coind_unfold TESL_interpretation_stepwise_cons_morph
-        by blast
-    then show ?thesis
-      by auto
+    have \<open>\<lbrakk> \<lceil>#\<^sup>\<le> K\<^sub>2 n, #\<^sup>\<le> K\<^sub>1 n\<rceil> \<in> (\<lambda>(x,y). x\<le>y) \<rbrakk>\<^sub>p\<^sub>r\<^sub>i\<^sub>m
+            \<inter> \<lbrakk> K\<^sub>1 weakly precedes K\<^sub>2 \<rbrakk>\<^sub>T\<^sub>E\<^sub>S\<^sub>L\<^bsup>\<ge> Suc n\<^esup> \<inter> \<lbrakk>\<lbrakk> \<Psi> \<rbrakk>\<rbrakk>\<^sub>T\<^sub>E\<^sub>S\<^sub>L\<^bsup>\<ge> n\<^esup>
+          = \<lbrakk>\<lbrakk> (K\<^sub>1 weakly precedes K\<^sub>2) # \<Psi> \<rbrakk>\<rbrakk>\<^sub>T\<^sub>E\<^sub>S\<^sub>L\<^bsup>\<ge> n\<^esup>\<close>
+      using TESL_interp_stepwise_weakly_precedes_coind_unfold
+            TESL_interpretation_stepwise_cons_morph by blast
+    thus ?thesis by auto
   qed
 qed
 
 lemma HeronConf_interp_stepwise_strictly_precedes_cases:
-  shows \<open>\<lbrakk> \<Gamma>, n \<turnstile> ((K\<^sub>1 strictly precedes K\<^sub>2) # \<Psi>) \<triangleright> \<Phi> \<rbrakk>\<^sub>c\<^sub>o\<^sub>n\<^sub>f\<^sub>i\<^sub>g
-          = \<lbrakk> ((\<lceil>#\<^sup>\<le> K\<^sub>2 n, #\<^sup>< K\<^sub>1 n\<rceil> \<in> (\<lambda>(x,y). x\<le>y)) # \<Gamma>), n \<turnstile> \<Psi> \<triangleright> ((K\<^sub>1 strictly precedes K\<^sub>2) # \<Phi>) \<rbrakk>\<^sub>c\<^sub>o\<^sub>n\<^sub>f\<^sub>i\<^sub>g\<close>
+   \<open>\<lbrakk> \<Gamma>, n \<turnstile> ((K\<^sub>1 strictly precedes K\<^sub>2) # \<Psi>) \<triangleright> \<Phi> \<rbrakk>\<^sub>c\<^sub>o\<^sub>n\<^sub>f\<^sub>i\<^sub>g
+    = \<lbrakk> ((\<lceil>#\<^sup>\<le> K\<^sub>2 n, #\<^sup>< K\<^sub>1 n\<rceil> \<in> (\<lambda>(x,y). x\<le>y)) # \<Gamma>), n
+      \<turnstile> \<Psi> \<triangleright> ((K\<^sub>1 strictly precedes K\<^sub>2) # \<Phi>) \<rbrakk>\<^sub>c\<^sub>o\<^sub>n\<^sub>f\<^sub>i\<^sub>g\<close>
 proof -
-  have \<open>\<lbrakk> \<Gamma>, n \<turnstile> (K\<^sub>1 strictly precedes K\<^sub>2) # \<Psi> \<triangleright> \<Phi> \<rbrakk>\<^sub>c\<^sub>o\<^sub>n\<^sub>f\<^sub>i\<^sub>g = \<lbrakk>\<lbrakk> \<Gamma> \<rbrakk>\<rbrakk>\<^sub>p\<^sub>r\<^sub>i\<^sub>m \<inter> \<lbrakk>\<lbrakk> (K\<^sub>1 strictly precedes K\<^sub>2) # \<Psi> \<rbrakk>\<rbrakk>\<^sub>T\<^sub>E\<^sub>S\<^sub>L\<^bsup>\<ge> n\<^esup> \<inter> \<lbrakk>\<lbrakk> \<Phi> \<rbrakk>\<rbrakk>\<^sub>T\<^sub>E\<^sub>S\<^sub>L\<^bsup>\<ge> Suc n\<^esup>\<close>
-    by simp
-  moreover have \<open>\<lbrakk> ((\<lceil>#\<^sup>\<le> K\<^sub>2 n, #\<^sup>< K\<^sub>1 n\<rceil> \<in> (\<lambda>(x,y). x\<le>y)) # \<Gamma>), n \<turnstile> \<Psi> \<triangleright> ((K\<^sub>1 strictly precedes K\<^sub>2) # \<Phi>) \<rbrakk>\<^sub>c\<^sub>o\<^sub>n\<^sub>f\<^sub>i\<^sub>g
-                    = \<lbrakk>\<lbrakk> (\<lceil>#\<^sup>\<le> K\<^sub>2 n, #\<^sup>< K\<^sub>1 n\<rceil> \<in> (\<lambda>(x,y). x\<le>y)) # \<Gamma> \<rbrakk>\<rbrakk>\<^sub>p\<^sub>r\<^sub>i\<^sub>m \<inter> \<lbrakk>\<lbrakk> \<Psi> \<rbrakk>\<rbrakk>\<^sub>T\<^sub>E\<^sub>S\<^sub>L\<^bsup>\<ge> n\<^esup> \<inter> \<lbrakk>\<lbrakk> (K\<^sub>1 strictly precedes K\<^sub>2) # \<Phi> \<rbrakk>\<rbrakk>\<^sub>T\<^sub>E\<^sub>S\<^sub>L\<^bsup>\<ge> Suc n\<^esup>\<close>
-    by simp
+  have \<open>\<lbrakk> \<Gamma>, n \<turnstile> (K\<^sub>1 strictly precedes K\<^sub>2) # \<Psi> \<triangleright> \<Phi> \<rbrakk>\<^sub>c\<^sub>o\<^sub>n\<^sub>f\<^sub>i\<^sub>g
+        = \<lbrakk>\<lbrakk> \<Gamma> \<rbrakk>\<rbrakk>\<^sub>p\<^sub>r\<^sub>i\<^sub>m \<inter> \<lbrakk>\<lbrakk> (K\<^sub>1 strictly precedes K\<^sub>2) # \<Psi> \<rbrakk>\<rbrakk>\<^sub>T\<^sub>E\<^sub>S\<^sub>L\<^bsup>\<ge> n\<^esup>
+          \<inter> \<lbrakk>\<lbrakk> \<Phi> \<rbrakk>\<rbrakk>\<^sub>T\<^sub>E\<^sub>S\<^sub>L\<^bsup>\<ge> Suc n\<^esup>\<close> by simp
+  moreover have \<open>\<lbrakk> ((\<lceil>#\<^sup>\<le> K\<^sub>2 n, #\<^sup>< K\<^sub>1 n\<rceil> \<in> (\<lambda>(x,y). x\<le>y)) # \<Gamma>), n
+                  \<turnstile> \<Psi> \<triangleright> ((K\<^sub>1 strictly precedes K\<^sub>2) # \<Phi>) \<rbrakk>\<^sub>c\<^sub>o\<^sub>n\<^sub>f\<^sub>i\<^sub>g
+                = \<lbrakk>\<lbrakk> (\<lceil>#\<^sup>\<le> K\<^sub>2 n, #\<^sup>< K\<^sub>1 n\<rceil> \<in> (\<lambda>(x,y). x\<le>y)) # \<Gamma> \<rbrakk>\<rbrakk>\<^sub>p\<^sub>r\<^sub>i\<^sub>m
+                \<inter> \<lbrakk>\<lbrakk> \<Psi> \<rbrakk>\<rbrakk>\<^sub>T\<^sub>E\<^sub>S\<^sub>L\<^bsup>\<ge> n\<^esup>
+                \<inter> \<lbrakk>\<lbrakk> (K\<^sub>1 strictly precedes K\<^sub>2) # \<Phi> \<rbrakk>\<rbrakk>\<^sub>T\<^sub>E\<^sub>S\<^sub>L\<^bsup>\<ge> Suc n\<^esup>\<close> by simp
   ultimately show ?thesis
   proof -
-    have \<open>\<lbrakk> \<lceil>#\<^sup>\<le> K\<^sub>2 n, #\<^sup>< K\<^sub>1 n\<rceil> \<in> (\<lambda>(x,y). x\<le>y) \<rbrakk>\<^sub>p\<^sub>r\<^sub>i\<^sub>m \<inter> \<lbrakk> K\<^sub>1 strictly precedes K\<^sub>2 \<rbrakk>\<^sub>T\<^sub>E\<^sub>S\<^sub>L\<^bsup>\<ge> Suc n\<^esup> \<inter> \<lbrakk>\<lbrakk> \<Psi> \<rbrakk>\<rbrakk>\<^sub>T\<^sub>E\<^sub>S\<^sub>L\<^bsup>\<ge> n\<^esup> = \<lbrakk>\<lbrakk> (K\<^sub>1 strictly precedes K\<^sub>2) # \<Psi> \<rbrakk>\<rbrakk>\<^sub>T\<^sub>E\<^sub>S\<^sub>L\<^bsup>\<ge> n\<^esup>\<close>
-      using TESL_interp_stepwise_strictly_precedes_coind_unfold TESL_interpretation_stepwise_cons_morph
-        by blast
-    then show ?thesis
-      by auto
+    have \<open>\<lbrakk> \<lceil>#\<^sup>\<le> K\<^sub>2 n, #\<^sup>< K\<^sub>1 n\<rceil> \<in> (\<lambda>(x,y). x\<le>y) \<rbrakk>\<^sub>p\<^sub>r\<^sub>i\<^sub>m
+            \<inter> \<lbrakk> K\<^sub>1 strictly precedes K\<^sub>2 \<rbrakk>\<^sub>T\<^sub>E\<^sub>S\<^sub>L\<^bsup>\<ge> Suc n\<^esup> \<inter> \<lbrakk>\<lbrakk> \<Psi> \<rbrakk>\<rbrakk>\<^sub>T\<^sub>E\<^sub>S\<^sub>L\<^bsup>\<ge> n\<^esup>
+          = \<lbrakk>\<lbrakk> (K\<^sub>1 strictly precedes K\<^sub>2) # \<Psi> \<rbrakk>\<rbrakk>\<^sub>T\<^sub>E\<^sub>S\<^sub>L\<^bsup>\<ge> n\<^esup>\<close>
+      using TESL_interp_stepwise_strictly_precedes_coind_unfold
+            TESL_interpretation_stepwise_cons_morph by blast
+    thus ?thesis by auto
   qed
 qed
 
 lemma HeronConf_interp_stepwise_kills_cases:
-  shows \<open>\<lbrakk> \<Gamma>, n \<turnstile> ((K\<^sub>1 kills K\<^sub>2) # \<Psi>) \<triangleright> \<Phi> \<rbrakk>\<^sub>c\<^sub>o\<^sub>n\<^sub>f\<^sub>i\<^sub>g
-          = \<lbrakk> ((K\<^sub>1 \<not>\<Up> n) # \<Gamma>), n \<turnstile> \<Psi> \<triangleright> ((K\<^sub>1 kills K\<^sub>2) # \<Phi>) \<rbrakk>\<^sub>c\<^sub>o\<^sub>n\<^sub>f\<^sub>i\<^sub>g
-          \<union> \<lbrakk> ((K\<^sub>1 \<Up> n) # (K\<^sub>2 \<not>\<Up> \<ge> n) # \<Gamma>), n \<turnstile> \<Psi> \<triangleright> ((K\<^sub>1 kills K\<^sub>2) # \<Phi>) \<rbrakk>\<^sub>c\<^sub>o\<^sub>n\<^sub>f\<^sub>i\<^sub>g\<close>
+   \<open>\<lbrakk> \<Gamma>, n \<turnstile> ((K\<^sub>1 kills K\<^sub>2) # \<Psi>) \<triangleright> \<Phi> \<rbrakk>\<^sub>c\<^sub>o\<^sub>n\<^sub>f\<^sub>i\<^sub>g
+    = \<lbrakk> ((K\<^sub>1 \<not>\<Up> n) # \<Gamma>), n \<turnstile> \<Psi> \<triangleright> ((K\<^sub>1 kills K\<^sub>2) # \<Phi>) \<rbrakk>\<^sub>c\<^sub>o\<^sub>n\<^sub>f\<^sub>i\<^sub>g
+    \<union> \<lbrakk> ((K\<^sub>1 \<Up> n) # (K\<^sub>2 \<not>\<Up> \<ge> n) # \<Gamma>), n \<turnstile> \<Psi> \<triangleright> ((K\<^sub>1 kills K\<^sub>2) # \<Phi>) \<rbrakk>\<^sub>c\<^sub>o\<^sub>n\<^sub>f\<^sub>i\<^sub>g\<close>
 proof -
-  have \<open>\<lbrakk> \<Gamma>, n \<turnstile> ((K\<^sub>1 kills K\<^sub>2) # \<Psi>) \<triangleright> \<Phi> \<rbrakk>\<^sub>c\<^sub>o\<^sub>n\<^sub>f\<^sub>i\<^sub>g = \<lbrakk>\<lbrakk> \<Gamma> \<rbrakk>\<rbrakk>\<^sub>p\<^sub>r\<^sub>i\<^sub>m \<inter> \<lbrakk>\<lbrakk> (K\<^sub>1 kills K\<^sub>2) # \<Psi> \<rbrakk>\<rbrakk>\<^sub>T\<^sub>E\<^sub>S\<^sub>L\<^bsup>\<ge> n\<^esup> \<inter> \<lbrakk>\<lbrakk> \<Phi> \<rbrakk>\<rbrakk>\<^sub>T\<^sub>E\<^sub>S\<^sub>L\<^bsup>\<ge> Suc n\<^esup>\<close>
+  have \<open>\<lbrakk> \<Gamma>, n \<turnstile> ((K\<^sub>1 kills K\<^sub>2) # \<Psi>) \<triangleright> \<Phi> \<rbrakk>\<^sub>c\<^sub>o\<^sub>n\<^sub>f\<^sub>i\<^sub>g
+        = \<lbrakk>\<lbrakk> \<Gamma> \<rbrakk>\<rbrakk>\<^sub>p\<^sub>r\<^sub>i\<^sub>m \<inter> \<lbrakk>\<lbrakk> (K\<^sub>1 kills K\<^sub>2) # \<Psi> \<rbrakk>\<rbrakk>\<^sub>T\<^sub>E\<^sub>S\<^sub>L\<^bsup>\<ge> n\<^esup> \<inter> \<lbrakk>\<lbrakk> \<Phi> \<rbrakk>\<rbrakk>\<^sub>T\<^sub>E\<^sub>S\<^sub>L\<^bsup>\<ge> Suc n\<^esup>\<close>
     by simp
   moreover have \<open>\<lbrakk> ((K\<^sub>1 \<not>\<Up> n) # \<Gamma>), n \<turnstile> \<Psi> \<triangleright> ((K\<^sub>1 kills K\<^sub>2) # \<Phi>) \<rbrakk>\<^sub>c\<^sub>o\<^sub>n\<^sub>f\<^sub>i\<^sub>g
-                = \<lbrakk>\<lbrakk> (K\<^sub>1 \<not>\<Up> n) # \<Gamma> \<rbrakk>\<rbrakk>\<^sub>p\<^sub>r\<^sub>i\<^sub>m \<inter> \<lbrakk>\<lbrakk> \<Psi> \<rbrakk>\<rbrakk>\<^sub>T\<^sub>E\<^sub>S\<^sub>L\<^bsup>\<ge> n\<^esup> \<inter> \<lbrakk>\<lbrakk> (K\<^sub>1 kills K\<^sub>2) # \<Phi> \<rbrakk>\<rbrakk>\<^sub>T\<^sub>E\<^sub>S\<^sub>L\<^bsup>\<ge> Suc n\<^esup>\<close>
-    by simp
+                = \<lbrakk>\<lbrakk> (K\<^sub>1 \<not>\<Up> n) # \<Gamma> \<rbrakk>\<rbrakk>\<^sub>p\<^sub>r\<^sub>i\<^sub>m \<inter> \<lbrakk>\<lbrakk> \<Psi> \<rbrakk>\<rbrakk>\<^sub>T\<^sub>E\<^sub>S\<^sub>L\<^bsup>\<ge> n\<^esup>
+                  \<inter> \<lbrakk>\<lbrakk> (K\<^sub>1 kills K\<^sub>2) # \<Phi> \<rbrakk>\<rbrakk>\<^sub>T\<^sub>E\<^sub>S\<^sub>L\<^bsup>\<ge> Suc n\<^esup>\<close> by simp
   moreover have \<open>\<lbrakk> ((K\<^sub>1 \<Up> n) # (K\<^sub>2 \<not>\<Up> \<ge> n) # \<Gamma>), n \<turnstile> \<Psi> \<triangleright> ((K\<^sub>1 kills K\<^sub>2) # \<Phi>) \<rbrakk>\<^sub>c\<^sub>o\<^sub>n\<^sub>f\<^sub>i\<^sub>g
-                = \<lbrakk>\<lbrakk> (K\<^sub>1 \<Up> n) # (K\<^sub>2 \<not>\<Up> \<ge> n) # \<Gamma> \<rbrakk>\<rbrakk>\<^sub>p\<^sub>r\<^sub>i\<^sub>m \<inter> \<lbrakk>\<lbrakk> \<Psi> \<rbrakk>\<rbrakk>\<^sub>T\<^sub>E\<^sub>S\<^sub>L\<^bsup>\<ge> n\<^esup> \<inter> \<lbrakk>\<lbrakk> (K\<^sub>1 kills K\<^sub>2) # \<Phi> \<rbrakk>\<rbrakk>\<^sub>T\<^sub>E\<^sub>S\<^sub>L\<^bsup>\<ge> Suc n\<^esup>\<close>
-  by simp
+                = \<lbrakk>\<lbrakk> (K\<^sub>1 \<Up> n) # (K\<^sub>2 \<not>\<Up> \<ge> n) # \<Gamma> \<rbrakk>\<rbrakk>\<^sub>p\<^sub>r\<^sub>i\<^sub>m \<inter> \<lbrakk>\<lbrakk> \<Psi> \<rbrakk>\<rbrakk>\<^sub>T\<^sub>E\<^sub>S\<^sub>L\<^bsup>\<ge> n\<^esup>
+                  \<inter> \<lbrakk>\<lbrakk> (K\<^sub>1 kills K\<^sub>2) # \<Phi> \<rbrakk>\<rbrakk>\<^sub>T\<^sub>E\<^sub>S\<^sub>L\<^bsup>\<ge> Suc n\<^esup>\<close> by simp
   ultimately show ?thesis
     proof -
-      have \<open>\<lbrakk>\<lbrakk> (K\<^sub>1 kills K\<^sub>2) # \<Psi> \<rbrakk>\<rbrakk>\<^sub>T\<^sub>E\<^sub>S\<^sub>L\<^bsup>\<ge> n\<^esup> = (\<lbrakk> (K\<^sub>1 \<not>\<Up> n) \<rbrakk>\<^sub>p\<^sub>r\<^sub>i\<^sub>m \<union> \<lbrakk> (K\<^sub>1 \<Up> n) \<rbrakk>\<^sub>p\<^sub>r\<^sub>i\<^sub>m \<inter> \<lbrakk> (K\<^sub>2 \<not>\<Up> \<ge> n) \<rbrakk>\<^sub>p\<^sub>r\<^sub>i\<^sub>m) \<inter> \<lbrakk> (K\<^sub>1 kills K\<^sub>2) \<rbrakk>\<^sub>T\<^sub>E\<^sub>S\<^sub>L\<^bsup>\<ge> Suc n\<^esup> \<inter> \<lbrakk>\<lbrakk> \<Psi> \<rbrakk>\<rbrakk>\<^sub>T\<^sub>E\<^sub>S\<^sub>L\<^bsup>\<ge> n\<^esup>\<close>
-        using TESL_interp_stepwise_kills_coind_unfold TESL_interpretation_stepwise_cons_morph
-        by blast
-      then show ?thesis
-        by auto
+      have \<open>\<lbrakk>\<lbrakk> (K\<^sub>1 kills K\<^sub>2) # \<Psi> \<rbrakk>\<rbrakk>\<^sub>T\<^sub>E\<^sub>S\<^sub>L\<^bsup>\<ge> n\<^esup>
+            = (\<lbrakk> (K\<^sub>1 \<not>\<Up> n) \<rbrakk>\<^sub>p\<^sub>r\<^sub>i\<^sub>m \<union> \<lbrakk> (K\<^sub>1 \<Up> n) \<rbrakk>\<^sub>p\<^sub>r\<^sub>i\<^sub>m \<inter> \<lbrakk> (K\<^sub>2 \<not>\<Up> \<ge> n) \<rbrakk>\<^sub>p\<^sub>r\<^sub>i\<^sub>m)
+              \<inter> \<lbrakk> (K\<^sub>1 kills K\<^sub>2) \<rbrakk>\<^sub>T\<^sub>E\<^sub>S\<^sub>L\<^bsup>\<ge> Suc n\<^esup> \<inter> \<lbrakk>\<lbrakk> \<Psi> \<rbrakk>\<rbrakk>\<^sub>T\<^sub>E\<^sub>S\<^sub>L\<^bsup>\<ge> n\<^esup>\<close>
+        using TESL_interp_stepwise_kills_coind_unfold
+              TESL_interpretation_stepwise_cons_morph by blast
+      thus ?thesis by auto
     qed
 qed
 
